# baseURI: https://www.gleif.org/ontology/Base/
# imports: https://www.omg.org/spec/LCC/Countries/CountryRepresentation/

@base <https://www.gleif.org/ontology/Base/> .
@prefix dct: <http://purl.org/dc/terms/> .
@prefix gleif-base: <https://www.gleif.org/ontology/Base/> .
@prefix lcc-cr: <https://www.omg.org/spec/LCC/Countries/CountryRepresentation/> .
@prefix owl: <http://www.w3.org/2002/07/owl#> .
@prefix rdf: <http://www.w3.org/1999/02/22-rdf-syntax-ns#> .
@prefix rdfs: <http://www.w3.org/2000/01/rdf-schema#> .
@prefix skos: <http://www.w3.org/2004/02/skos/core#> .
@prefix vann: <http://purl.org/vocab/vann/> .
@prefix voaf: <http://purl.org/vocommons/voaf#> .
@prefix xml: <http://www.w3.org/XML/1998/namespace> .
@prefix xsd: <http://www.w3.org/2001/XMLSchema#> .

<https://www.gleif.org/ontology/Base/>
	a
		voaf:Vocabulary ,
		owl:Ontology
		;
	rdfs:label "GLEIF Base Ontology"@en ;
	dct:abstract "Ontology defining generic concepts for reuse by other Global Legal Entity Identifier Foundation (GLEIF) ontologies. It defines generic classes for (legal) Entities and their relationships and statuses; and generic properties for different types of name and address. It makes use of the OMG Languages Countries and Codes (LCC) ontology (based on the ISO 3166 standard) for country and region information."@en ;
	dct:contributor
		<http://purl.org/bryon> ,
		<http://www.workingontologist.com> ,
		<https://www.linkedin.com/in/peterivett/>
		;
	dct:creator gleif-base:GLEIF ;
	dct:issued "2019-02-01T00:00:00Z"^^xsd:dateTime ;
	dct:license "https://www.gleif.org/en/meta/lei-data-terms-of-use/"^^xsd:anyURI ;
	dct:rights "Copyright (c) 2019 Global Legal Entity Identifier Foundation (GLEIF)" ;
	dct:rightsHolder gleif-base:GLEIF ;
	dct:source "https://www.gleif.org/en/about-lei/common-data-file-format/lei-cdf-format/lei-cdf-format-version-2-1"^^xsd:anyURI ;
	dct:title "Global Legal Entity Identifier Foundation Base Ontology"@en ;
	vann:preferredNamespacePrefix "gleif-base" ;
	vann:preferredNamespaceUri "https://www.gleif.org/ontology/Base/" ;
	owl:imports <https://www.omg.org/spec/LCC/Countries/CountryRepresentation/> ;
	owl:versionIRI <https://www.gleif.org/ontology/Base-v1.0/Base/> ;
	.

gleif-base:Entity
	a owl:Class ;
	rdfs:subClassOf
		[
			a owl:Restriction ;
			owl:onProperty gleif-base:hasNameLegalLocal ;
			owl:cardinality "1"^^xsd:nonNegativeInteger ;
		] ,
		[
			a owl:Restriction ;
			owl:onProperty gleif-base:hasEntityExpirationReason ;
			owl:onClass gleif-base:EntityExpirationReason ;
			owl:maxQualifiedCardinality "1"^^xsd:nonNegativeInteger ;
		] ,
		[
			a owl:Restriction ;
			owl:onProperty gleif-base:hasEntityExpirationDate ;
			owl:maxQualifiedCardinality "1"^^xsd:nonNegativeInteger ;
			owl:onDataRange xsd:dateTime ;
		] ,
		[
			a owl:Restriction ;
			owl:onProperty gleif-base:hasSuccessor ;
			owl:onClass gleif-base:Entity ;
			owl:minQualifiedCardinality "0"^^xsd:nonNegativeInteger ;
		] ,
		[
			a owl:Restriction ;
			owl:onProperty gleif-base:hasLegalJurisdiction ;
			owl:onClass lcc-cr:GeographicRegion ;
			owl:minQualifiedCardinality "0"^^xsd:nonNegativeInteger ;
		] ,
		[
			a owl:Restriction ;
			owl:onProperty gleif-base:hasEntityStatus ;
			owl:onClass gleif-base:EntityStatus ;
			owl:qualifiedCardinality "1"^^xsd:nonNegativeInteger ;
		]
		;
	rdfs:label "entity" ;
	rdfs:isDefinedBy <https://www.gleif.org/ontology/Base/> ;
	skos:definition "A partnership, corporation, or other organization having the capacity to negotiate contracts, assume financial obligations, and pay off debts, organized under the laws of some jurisdiction." ;
	.

gleif-base:EntityExpirationReason
	a owl:Class ;
	rdfs:label "entity expiration reason" ;
	rdfs:isDefinedBy <https://www.gleif.org/ontology/Base/> ;
	owl:oneOf (
		gleif-base:EntityExpirationReasonCorporateAction
		gleif-base:EntityExpirationReasonDissolved
		gleif-base:EntityExpirationReasonOther
	) ;
	skos:definition "The reason that an entity ceased to exist and/or operate." ;
	.

gleif-base:EntityExpirationReasonCorporateAction
	a gleif-base:EntityExpirationReason ;
	rdfs:label "corporate action" ;
	rdfs:isDefinedBy <https://www.gleif.org/ontology/Base/> ;
	skos:definition "The entity was acquired or merged with another entity." ;
	gleif-base:hasTag "CORPORATE_ACTION" ;
	.

gleif-base:EntityExpirationReasonDissolved
	a gleif-base:EntityExpirationReason ;
	rdfs:label "dissolved" ;
	rdfs:isDefinedBy <https://www.gleif.org/ontology/Base/> ;
	skos:definition "The entity ceased to operate." ;
	gleif-base:hasTag "DISSOLVED" ;
	.

gleif-base:EntityExpirationReasonOther
	a gleif-base:EntityExpirationReason ;
	rdfs:label "other" ;
	rdfs:isDefinedBy <https://www.gleif.org/ontology/Base/> ;
	skos:definition "The reason for expiry is neither of dissolved nor corporate action." ;
	gleif-base:hasTag "OTHER" ;
	.

gleif-base:EntityStatus
	a owl:Class ;
	rdfs:label "entity status" ;
	rdfs:isDefinedBy <https://www.gleif.org/ontology/Base/> ;
	owl:oneOf (
		gleif-base:EntityStatusActive
		gleif-base:EntityStatusInactive
	) ;
	skos:definition "The operational and/or legal registration status of the entity (may be ACTIVE or INACTIVE)" ;
	.

gleif-base:EntityStatusActive
	a
		owl:NamedIndividual ,
		gleif-base:EntityStatus
		;
	rdfs:label "active" ;
	rdfs:isDefinedBy <https://www.gleif.org/ontology/Base/> ;
	skos:definition "As of the last report or update, the entity reported that it was legally registered and operating." ;
	gleif-base:hasTag "ACTIVE" ;
	.

gleif-base:EntityStatusInactive
	a
		owl:NamedIndividual ,
		gleif-base:EntityStatus
		;
	rdfs:label "inactive" ;
	rdfs:isDefinedBy <https://www.gleif.org/ontology/Base/> ;
	skos:definition "It has been determined that the entity that was assigned the LEI is no longer legally registered and/or operating, whether as a result of business closure, acquisition by or merger with another (or new) entity, or determination of illegitimacy." ;
	gleif-base:hasTag "INACTIVE" ;
	.

gleif-base:GLEIF
	a gleif-base:RegistrationAuthority ;
	rdfs:isDefinedBy <https://www.gleif.org/ontology/Base/> ;
	gleif-base:hasLegalName "Global Legal Entity Identifier Foundation" ;
	gleif-base:hasNameLegalLocal "Global Legal Entity Identifier Foundation"@en ;
	.

gleif-base:Identifier
	a owl:Class ;
	rdfs:subClassOf
		[
			a owl:Restriction ;
			owl:onProperty gleif-base:identifies ;
			owl:cardinality "1"^^xsd:nonNegativeInteger ;
		] ,
		[
			a owl:Restriction ;
			owl:onProperty gleif-base:hasTag ;
			owl:onDataRange xsd:string ;
			owl:qualifiedCardinality "1"^^xsd:nonNegativeInteger ;
		]
		;
	rdfs:label "identifier" ;
	rdfs:isDefinedBy <https://www.gleif.org/ontology/Base/> ;
	skos:definition "Sequence of characters, capable of uniquely identifying that with which it is associated, within a specified context." ;
	.

gleif-base:LegalEntityRelationship
	a owl:Class ;
	rdfs:subClassOf
		[
			a owl:Restriction ;
			owl:onProperty gleif-base:hasSource ;
			owl:onClass gleif-base:Entity ;
			owl:qualifiedCardinality "1"^^xsd:nonNegativeInteger ;
		] ,
		[
			a owl:Restriction ;
			owl:onProperty gleif-base:hasTarget ;
			owl:onClass gleif-base:Entity ;
			owl:qualifiedCardinality "1"^^xsd:nonNegativeInteger ;
		]
		;
	rdfs:label "legal entity relationship" ;
	rdfs:isDefinedBy <https://www.gleif.org/ontology/Base/> ;
	skos:definition "abstract superclass to represent a reified directed relationship" ;
	.

gleif-base:LegalPerson
	a owl:Class ;
	rdfs:subClassOf gleif-base:Entity ;
	rdfs:label "legal person" ;
	rdfs:isDefinedBy <https://www.gleif.org/ontology/Base/> ;
	skos:definition "Any entity which can incur legal obligation and can be sued at law." ;
	.

gleif-base:Period
	a owl:Class ;
	rdfs:subClassOf
		[
			a owl:Restriction ;
			owl:onProperty gleif-base:hasEnd ;
			owl:maxQualifiedCardinality "1" ;
			owl:onDataRange xsd:dateTime ;
		] ,
		[
			a owl:Restriction ;
			owl:onProperty gleif-base:hasStart ;
			owl:onDataRange xsd:dateTime ;
			owl:qualifiedCardinality "1" ;
		]
		;
	rdfs:label "period"@en ;
	rdfs:isDefinedBy <https://www.gleif.org/ontology/Base/> ;
	skos:definition "A period of time, with at least a start time, and possibly an end." ;
	.

gleif-base:PhysicalAddress
	a owl:Class ;
	rdfs:subClassOf
		[
			a owl:Restriction ;
			owl:onProperty gleif-base:hasAddressLine1 ;
			owl:cardinality "1" ;
		] ,
		[
			a owl:Restriction ;
			owl:onProperty gleif-base:hasCity ;
			owl:cardinality "1" ;
		] ,
		[
			a owl:Restriction ;
			owl:onProperty gleif-base:hasAddressLine2 ;
			owl:maxCardinality "1" ;
		] ,
		[
			a owl:Restriction ;
			owl:onProperty gleif-base:hasAddressLine3 ;
			owl:maxCardinality "1" ;
		] ,
		[
			a owl:Restriction ;
			owl:onProperty gleif-base:hasAddressLine4 ;
			owl:maxCardinality "1" ;
		] ,
		[
			a owl:Restriction ;
			owl:onProperty gleif-base:hasAddressNumber ;
			owl:maxCardinality "1" ;
		] ,
		[
			a owl:Restriction ;
			owl:onProperty gleif-base:hasAddressNumberWithinBuilding ;
			owl:maxCardinality "1" ;
		] ,
		[
			a owl:Restriction ;
			owl:onProperty gleif-base:hasMailRouting ;
			owl:maxCardinality "1" ;
		] ,
		[
			a owl:Restriction ;
			owl:onProperty gleif-base:hasPostalCode ;
			owl:maxCardinality "1" ;
		] ,
		[
			a owl:Restriction ;
			owl:onProperty gleif-base:hasRegion ;
			owl:onClass lcc-cr:Region ;
			owl:maxQualifiedCardinality "1" ;
		] ,
		[
			a owl:Restriction ;
			owl:onProperty gleif-base:hasCountry ;
			owl:onClass lcc-cr:Country ;
			owl:qualifiedCardinality "1" ;
		]
		;
	rdfs:label "physical address"@en ;
	rdfs:isDefinedBy <https://www.gleif.org/ontology/Base/> ;
	skos:definition "a physical address where communications can be addressed, papers served or representatives located for any kind of organization or person" ;
	skos:note "An address is a collection of information, presented in a mostly fixed format, used for describing the location of a building, apartment, or other structure or a plot of land, generally using political boundaries and street names as references, along with other identifiers such as house or apartment numbers.  Some addresses also contain special codes to aid routing of mail and packages, such as a ZIP code or post code. (Wikipedia)" ;
	.

gleif-base:PhysicalAddressASCII
	a owl:Class ;
	rdfs:subClassOf gleif-base:PhysicalAddress ;
	rdfs:label "physical address ASCII" ;
	rdfs:isDefinedBy <https://www.gleif.org/ontology/Base/> ;
	skos:definition "An address transliterated to ASCII characters." ;
	.

gleif-base:RegistrationAuthority
	a owl:Class ;
	rdfs:subClassOf gleif-base:Entity ;
	rdfs:label "registration authority" ;
	rdfs:isDefinedBy <https://www.gleif.org/ontology/Base/> ;
	skos:altLabel "RA" ;
	skos:definition "An organization that is responsible for maintaining a registry and provides registration services." ;
	skos:prefLabel "registration authority" ;
	.

gleif-base:RegistrationStatus
	a owl:Class ;
	rdfs:label "registration status" ;
	rdfs:isDefinedBy <https://www.gleif.org/ontology/Base/> ;
	skos:definition "A lifecycle stage indicating the status of a given registration of something, such as a business or legal entity." ;
	.

gleif-base:Registry
	a owl:Class ;
	rdfs:subClassOf [
		a owl:Restriction ;
		owl:onProperty gleif-base:isManagedBy ;
		owl:onClass gleif-base:Entity ;
		owl:qualifiedCardinality "1"^^xsd:nonNegativeInteger ;
	] ;
	rdfs:label "registry" ;
	rdfs:isDefinedBy <https://www.gleif.org/ontology/Base/> ;
	skos:definition "A system, typically an information system, that records the registration of items." ;
	.

gleif-base:RegistryEntry
	a owl:Class ;
	rdfs:label "registry entry" ;
	rdfs:isDefinedBy <https://www.gleif.org/ontology/Base/> ;
	skos:definition "An entry in a registry that specifies something about the thing that is recorded." ;
	.

gleif-base:RegistryIdentifier
	a owl:Class ;
	rdfs:subClassOf
		gleif-base:Identifier ,
		[
			a owl:Restriction ;
			owl:onProperty gleif-base:isRegisteredIn ;
			owl:someValuesFrom gleif-base:Registry ;
		]
		;
	rdfs:label "registry identifier" ;
	rdfs:isDefinedBy <https://www.gleif.org/ontology/Base/> ;
	skos:definition "An identifier associated with an entry in a registry, i.e., one that provides an index to the registry for the recorded item." ;
	.

gleif-base:hasAbbreviation
	a owl:DatatypeProperty ;
	rdfs:subPropertyOf skos:altLabel ;
	rdfs:label "has abbreviation" ;
	rdfs:isDefinedBy <https://www.gleif.org/ontology/Base/> ;
	skos:definition "An abbreviation for the entity identified." ;
	.

gleif-base:hasAbbreviationLocal
	a owl:DatatypeProperty ;
	rdfs:subPropertyOf gleif-base:hasAbbreviation ;
	rdfs:label "has abbreviation local" ;
	rdfs:isDefinedBy <https://www.gleif.org/ontology/Base/> ;
	skos:definition "An abbreviation using a language local to the entity identified; may be English." ;
	.

gleif-base:hasAbbreviationTransliterated
	a owl:DatatypeProperty ;
	rdfs:subPropertyOf gleif-base:hasAbbreviation ;
	rdfs:label "has abbreviation transliterated" ;
	rdfs:isDefinedBy <https://www.gleif.org/ontology/Base/> ;
	skos:definition "An abbreviation transliterated into a Western alphabet." ;
	.

gleif-base:hasAdditionalAddressLine
	a owl:DatatypeProperty ;
	rdfs:label "has additional address line" ;
	rdfs:domain gleif-base:PhysicalAddress ;
	rdfs:isDefinedBy <https://www.gleif.org/ontology/Base/> ;
	skos:definition "Means to collect the one to three specifically-named optional additional address line elements." ;
	.

gleif-base:hasAddress
	a owl:ObjectProperty ;
	rdfs:label "has address" ;
	rdfs:domain gleif-base:Entity ;
	rdfs:isDefinedBy <https://www.gleif.org/ontology/Base/> ;
	rdfs:range gleif-base:PhysicalAddress ;
	skos:definition "Has a means by which the entity may be located or contacted or may receive correspondence." ;
	.

gleif-base:hasAddressHeadquarters
	a owl:ObjectProperty ;
	rdfs:subPropertyOf gleif-base:hasAddress ;
	rdfs:label "has address headquarters" ;
	rdfs:isDefinedBy <https://www.gleif.org/ontology/Base/> ;
	skos:definition "An address of the headquarters of the Entity." ;
	.

gleif-base:hasAddressLegal
	a owl:ObjectProperty ;
	rdfs:subPropertyOf gleif-base:hasAddress ;
	rdfs:label "has address legal" ;
	rdfs:isDefinedBy <https://www.gleif.org/ontology/Base/> ;
	skos:definition "An address of the entity as recorded in the registration of the entity in its legal jurisdiction." ;
	.

gleif-base:hasAddressLine1
	a owl:DatatypeProperty ;
	rdfs:label "has address line 1" ;
	rdfs:domain gleif-base:PhysicalAddress ;
	rdfs:isDefinedBy <https://www.gleif.org/ontology/Base/> ;
	skos:definition "The mandatory first address line element." ;
	.

gleif-base:hasAddressLine2
	a owl:DatatypeProperty ;
	rdfs:subPropertyOf gleif-base:hasAdditionalAddressLine ;
	rdfs:label "has address line 2" ;
	rdfs:domain gleif-base:PhysicalAddress ;
	rdfs:isDefinedBy <https://www.gleif.org/ontology/Base/> ;
	skos:definition "The second line of the one to three optional additional address line elements." ;
	.

gleif-base:hasAddressLine3
	a owl:DatatypeProperty ;
	rdfs:subPropertyOf gleif-base:hasAdditionalAddressLine ;
	rdfs:label "has address line 3" ;
	rdfs:domain gleif-base:PhysicalAddress ;
	rdfs:isDefinedBy <https://www.gleif.org/ontology/Base/> ;
	skos:definition "The third line of the one to three optional additional address line elements." ;
	skos:note "This element SHALL be omitted if address line 2 is omitted." ;
	.

gleif-base:hasAddressLine4
	a owl:DatatypeProperty ;
	rdfs:subPropertyOf gleif-base:hasAdditionalAddressLine ;
	rdfs:label "has address line 4" ;
	rdfs:domain gleif-base:PhysicalAddress ;
	rdfs:isDefinedBy <https://www.gleif.org/ontology/Base/> ;
	skos:definition "The fourth line of the one to three optional additional address line elements." ;
	skos:note "This element SHALL be omitted if address line 3 is omitted." ;
	.

gleif-base:hasAddressNumber
	a owl:DatatypeProperty ;
	rdfs:label "has address number" ;
	rdfs:domain gleif-base:PhysicalAddress ;
	rdfs:isDefinedBy <https://www.gleif.org/ontology/Base/> ;
	skos:definition "Optional, additional structured version of an external house number, or range of numbers, contained in one of the address line elements." ;
	.

gleif-base:hasAddressNumberWithinBuilding
	a owl:DatatypeProperty ;
	rdfs:label "has address number within building" ;
	rdfs:domain gleif-base:PhysicalAddress ;
	rdfs:isDefinedBy <https://www.gleif.org/ontology/Base/> ;
	skos:definition "Optional, additional structured version of an internal location number, or range of numbers, contained in one of the address line elements." ;
	.

gleif-base:hasAddressTransliterated
	a owl:ObjectProperty ;
	rdfs:subPropertyOf gleif-base:hasAddress ;
	rdfs:label "has address transliterated" ;
	rdfs:isDefinedBy <https://www.gleif.org/ontology/Base/> ;
	rdfs:range gleif-base:PhysicalAddressASCII ;
	skos:definition "An address which has been converted from original to western text." ;
	.

gleif-base:hasCity
	a owl:DatatypeProperty ;
	rdfs:label "has city" ;
	rdfs:domain gleif-base:PhysicalAddress ;
	rdfs:isDefinedBy <https://www.gleif.org/ontology/Base/> ;
	skos:definition "The mandatory name of the city." ;
	.

gleif-base:hasCountry
	a owl:ObjectProperty ;
	rdfs:subPropertyOf gleif-base:hasGeographicRegion ;
	rdfs:label "has country" ;
	rdfs:domain gleif-base:PhysicalAddress ;
	rdfs:isDefinedBy <https://www.gleif.org/ontology/Base/> ;
	rdfs:range lcc-cr:Country ;
	skos:definition "The country, based on the 2-character ISO 3166-1 country code." ;
	.

gleif-base:hasCoverageArea
	a owl:ObjectProperty ;
	rdfs:label "has coverage area" ;
	rdfs:isDefinedBy <https://www.gleif.org/ontology/Base/> ;
	rdfs:range lcc-cr:GeographicRegion ;
	skos:definition "Indicates a geographic region in which some service is provided, or to which some policy applies, or in which something is available." ;
	.

gleif-base:hasEnd
	a owl:DatatypeProperty ;
	rdfs:label "has end"@en ;
	rdfs:domain gleif-base:Period ;
	rdfs:isDefinedBy <https://www.gleif.org/ontology/Base/> ;
	rdfs:range xsd:dateTime ;
	skos:definition "The end time of a period." ;
	.

gleif-base:hasEntityExpirationDate
	a owl:DatatypeProperty ;
	rdfs:label "has entity expiration date" ;
	rdfs:domain gleif-base:Entity ;
	rdfs:isDefinedBy <https://www.gleif.org/ontology/Base/> ;
	rdfs:range xsd:dateTime ;
	skos:definition "The date that the entity ceased to operate, whether due to dissolution, merger or acquisition." ;
	.

gleif-base:hasEntityExpirationReason
	a owl:ObjectProperty ;
	rdfs:label "has entity expiration reason" ;
	rdfs:domain gleif-base:Entity ;
	rdfs:isDefinedBy <https://www.gleif.org/ontology/Base/> ;
	rdfs:range gleif-base:EntityExpirationReason ;
	skos:definition "The reason that an entity ceased to exist and/or operate." ;
	.

gleif-base:hasEntityStatus
	a
		owl:ObjectProperty ,
		owl:FunctionalProperty
		;
	rdfs:label "has entity status" ;
	rdfs:domain gleif-base:Entity ;
	rdfs:isDefinedBy <https://www.gleif.org/ontology/Base/> ;
	rdfs:range gleif-base:EntityStatus ;
	skos:definition "Indicates the status of the entity (i.e., active, inactive)." ;
	.

gleif-base:hasFirstAddressLine
	a owl:DatatypeProperty ;
	rdfs:label "has first address line" ;
	rdfs:domain gleif-base:PhysicalAddress ;
	rdfs:isDefinedBy <https://www.gleif.org/ontology/Base/> ;
	owl:equivalentProperty gleif-base:hasAddressLine1 ;
	skos:definition "The mandatory first address line element." ;
	.

gleif-base:hasGeographicRegion
	a owl:ObjectProperty ;
	rdfs:label "has geographic region" ;
	rdfs:isDefinedBy <https://www.gleif.org/ontology/Base/> ;
	rdfs:range lcc-cr:GeographicRegion ;
	skos:definition "The country or region where something is located." ;
	.

gleif-base:hasInitialRegistrationDate
	a owl:DatatypeProperty ;
	rdfs:subPropertyOf dct:created ;
	rdfs:label "has initial registration date" ;
	rdfs:isDefinedBy <https://www.gleif.org/ontology/Base/> ;
	rdfs:range xsd:dateTime ;
	skos:definition "The date on which an identifier or other registered item was first registered." ;
	.

gleif-base:hasLastUpdateDate
	a owl:DatatypeProperty ;
	rdfs:subPropertyOf dct:modified ;
	rdfs:label "has last modification date" ;
	rdfs:isDefinedBy <https://www.gleif.org/ontology/Base/> ;
	rdfs:range xsd:dateTime ;
	skos:definition "The date that the detail of a specific registration in the registry was last revised." ;
	.

gleif-base:hasLegalJurisdiction
	a owl:ObjectProperty ;
	rdfs:label "has legal jurisdiction" ;
	rdfs:domain gleif-base:Entity ;
	rdfs:isDefinedBy <https://www.gleif.org/ontology/Base/> ;
	rdfs:range lcc-cr:GeographicRegion ;
	skos:definition "The jurisdiction of legal formation and registration of the entity (and upon which the LegalForm data element is also dependent). " ;
	.

gleif-base:hasMailRouting
	a owl:DatatypeProperty ;
	rdfs:label "mail routing" ;
	rdfs:domain gleif-base:PhysicalAddress ;
	rdfs:isDefinedBy <https://www.gleif.org/ontology/Base/> ;
	skos:definition "Optional free text address line to hold content from other address lines containing explicit routing information (this element's presence indicates that this address is a routing / 'care of' address)." ;
	.

gleif-base:hasName
	a owl:DatatypeProperty ;
	rdfs:subPropertyOf rdfs:label ;
	rdfs:label "has name" ;
	rdfs:isDefinedBy <https://www.gleif.org/ontology/Base/> ;
	skos:definition "Associates a name, reference name, or appellation with an individual resource." ;
	.

gleif-base:hasNameASCII
	a owl:DatatypeProperty ;
	rdfs:subPropertyOf gleif-base:hasNameTransliterated ;
	rdfs:label "has name ASCII" ;
	rdfs:isDefinedBy <https://www.gleif.org/ontology/Base/> ;
	skos:altLabel "has ASCII name" ;
	skos:definition "The name used to refer to a person or organization in 7 bit ASCII text (ISO 646); also valid UNICODE (ISO 10646)." ;
	skos:prefLabel "has name ASCII" ;
	.

gleif-base:hasNameASCIIAutomatic
	a owl:DatatypeProperty ;
	rdfs:subPropertyOf
		gleif-base:hasNameASCII ,
		gleif-base:hasNameLegal
		;
	rdfs:label "has name ASCII automatic" ;
	rdfs:isDefinedBy <https://www.gleif.org/ontology/Base/> ;
	skos:altLabel "has auto ASCII transliterated legal name" ;
	skos:definition "Legal name of the entity transliterated to ASCII characters, auto-transliterated by the managing LOU." ;
	skos:prefLabel "has name ASCII automatic" ;
	.

gleif-base:hasNameASCIIPreferred
	a owl:DatatypeProperty ;
	rdfs:subPropertyOf
		gleif-base:hasNameASCII ,
		gleif-base:hasNameLegal
		;
	rdfs:label "has name ASCII preferred" ;
	rdfs:isDefinedBy <https://www.gleif.org/ontology/Base/> ;
	skos:altLabel "has preferred transliterated legal name" ;
	skos:definition "Legal name of the entity transliterated to ASCII characters, provided by the entity for this purpose." ;
	skos:prefLabel "has name ASCII preferred" ;
	.

gleif-base:hasNameAdditional
	a owl:DatatypeProperty ;
	rdfs:subPropertyOf
		skos:altLabel ,
		gleif-base:hasName
		;
	rdfs:label "has name additional" ;
	rdfs:isDefinedBy <https://www.gleif.org/ontology/Base/> ;
	skos:altLabel "has other name" ;
	skos:definition "The name used to refer to an person or organization informally." ;
	skos:prefLabel "has name additional" ;
	.

gleif-base:hasNameAdditionalLocal
	a owl:DatatypeProperty ;
	rdfs:subPropertyOf
		gleif-base:hasNameAdditional ,
		gleif-base:hasNameLocal
		;
	rdfs:label "has name additional local" ;
	rdfs:isDefinedBy <https://www.gleif.org/ontology/Base/> ;
	skos:definition "Registered name of the entity in an alternative language in the legal jurisdiction in which the entity is registered." ;
	.

gleif-base:hasNameLegal
	a owl:DatatypeProperty ;
	rdfs:subPropertyOf gleif-base:hasName ;
	rdfs:label "has name legal" ;
	rdfs:isDefinedBy <https://www.gleif.org/ontology/Base/> ;
	skos:altLabel "has legal name" ;
	skos:definition "The name used to refer to an person or organization in legal communications." ;
	skos:prefLabel "has name legal" ;
	.

gleif-base:hasNameLegalLocal
	a owl:DatatypeProperty ;
	rdfs:subPropertyOf
		skos:prefLabel ,
		gleif-base:hasNameLegal ,
		gleif-base:hasNameLocal
		;
	rdfs:label "has name legal local" ;
	rdfs:isDefinedBy <https://www.gleif.org/ontology/Base/> ;
	skos:altLabel "has local legal name" ;
	skos:definition "The name used to refer to an person or organization in legal communications in local alphabet, which may be English." ;
	skos:prefLabel "has name legal local" ;
	.

gleif-base:hasNameLocal
	a owl:DatatypeProperty ;
	rdfs:subPropertyOf gleif-base:hasName ;
	rdfs:label "has name local" ;
	rdfs:isDefinedBy <https://www.gleif.org/ontology/Base/> ;
	skos:altLabel "has local name" ;
	skos:definition "A name in a language local to the entity identified; may be English." ;
	skos:prefLabel "has name local" ;
	.

gleif-base:hasNamePreviousLegal
	a owl:DatatypeProperty ;
	rdfs:subPropertyOf gleif-base:hasNameAdditional ;
	rdfs:label "has name previous legal" ;
	rdfs:isDefinedBy <https://www.gleif.org/ontology/base/> ;
	skos:definition "A primary legal name previously used by this entity." ;
	.

gleif-base:hasNameTradingOrOperating
	a owl:DatatypeProperty ;
	rdfs:subPropertyOf gleif-base:hasNameAdditional ;
	rdfs:label "has name trading or operating" ;
	rdfs:isDefinedBy <https://www.gleif.org/ontology/base/> ;
	skos:altLabel
		"brand name" ,
		"doing business as" ,
		"has trading or operating name" ,
		"operating under" ,
		"trading as"
		;
	skos:definition "A 'trading as', 'brand name' or 'operating under' name currently used by this entity in addition to, but not replacing, the (primary) legal, official registered name" ;
	skos:prefLabel "has name trading or operating" ;
	.

gleif-base:hasNameTranslatedEnglish
	a owl:DatatypeProperty ;
	rdfs:subPropertyOf gleif-base:hasNameASCII ;
	rdfs:label "has name translated English" ;
	rdfs:isDefinedBy <https://www.gleif.org/ontology/Base/> ;
	skos:altLabel
		"has English name" ,
		"has international name"
		;
	skos:definition "The name used to refer to a person or organization, translated into English. Transliterated to ASCII by definition." ;
	skos:prefLabel "has name translated English" ;
	.

gleif-base:hasNameTransliterated
	a owl:DatatypeProperty ;
	rdfs:subPropertyOf
		skos:altLabel ,
		gleif-base:hasName
		;
	rdfs:label "has name transliterated" ;
	rdfs:isDefinedBy <https://www.gleif.org/ontology/Base/> ;
	skos:altLabel
		"has transliterated name" ,
		"has transliterated other names"
		;
	skos:definition "The name used to refer to a person or organization, converted from original to western text. Not generally the legal name." ;
	skos:prefLabel "has name transliterated" ;
	.

gleif-base:hasNextRenewalDate
	a owl:DatatypeProperty ;
	rdfs:label "has next renewal date" ;
	rdfs:isDefinedBy <https://www.gleif.org/ontology/Base/> ;
	rdfs:range xsd:dateTime ;
	skos:definition "The date by which a specific registration in the registry must be renewed or updated." ;
	.

gleif-base:hasPostalCode
	a owl:DatatypeProperty ;
	rdfs:label "has postal code" ;
	rdfs:domain gleif-base:PhysicalAddress ;
	rdfs:isDefinedBy <https://www.gleif.org/ontology/Base/> ;
	skos:definition "The (optional) postal code of this address as specified by the local postal service." ;
	.

gleif-base:hasRegion
	a owl:ObjectProperty ;
	rdfs:subPropertyOf gleif-base:hasGeographicRegion ;
	rdfs:label "has region" ;
	rdfs:isDefinedBy <https://www.gleif.org/ontology/Base/> ;
	rdfs:range lcc-cr:CountrySubdivision ;
	skos:altLabel
		"has state" ,
		"has subdivision"
		;
	skos:definition "The (optional) region or subdivision (state, province, region, etc.) based on the 4- to 6-character ISO 3166-2 region code" ;
	skos:prefLabel "has region" ;
	.

gleif-base:hasRegistrationStatus
	a
		owl:ObjectProperty ,
		owl:FunctionalProperty
		;
	rdfs:label "has registration status" ;
	rdfs:isDefinedBy <https://www.gleif.org/ontology/Base/> ;
	rdfs:range gleif-base:RegistrationStatus ;
	skos:definition "indicates the status of a specific registration, such as for an identifier or license" ;
	.

gleif-base:hasSource
	a
		owl:ObjectProperty ,
		owl:FunctionalProperty
		;
	rdfs:label "has source" ;
	rdfs:domain gleif-base:LegalEntityRelationship ;
	rdfs:isDefinedBy <https://www.gleif.org/ontology/Base/> ;
	rdfs:range gleif-base:Entity ;
	skos:definition "The entity that is the source of the directed relationship." ;
	.

gleif-base:hasStart
	a owl:DatatypeProperty ;
	rdfs:label "has start"@en ;
	rdfs:domain gleif-base:Period ;
	rdfs:isDefinedBy <https://www.gleif.org/ontology/Base/> ;
	rdfs:range xsd:dateTime ;
	skos:definition "The start time of a period." ;
	.

gleif-base:hasSuccessor
	a owl:ObjectProperty ;
	rdfs:label "has successor" ;
	rdfs:domain gleif-base:Entity ;
	rdfs:isDefinedBy <https://www.gleif.org/ontology/Base/> ;
	rdfs:range gleif-base:Entity ;
	skos:definition "The surviving/new entity which continues/replaces this registration." ;
	.

gleif-base:hasSuccessorName
	a owl:DatatypeProperty ;
	rdfs:label "has successor name" ;
	rdfs:domain gleif-base:Entity ;
	rdfs:isDefinedBy <https://www.gleif.org/ontology/Base/> ;
	skos:definition "The name of the successor entity." ;
	.

gleif-base:hasTag
	a
		owl:DatatypeProperty ,
		owl:FunctionalProperty
		;
	rdfs:subPropertyOf skos:notation ;
	rdfs:label "has tag" ;
	rdfs:isDefinedBy <https://www.gleif.org/ontology/Base/> ;
	rdfs:range xsd:string ;
	skos:definition "Has a unique combination of alphanumeric characters or binary representation corresponding to the identifier, code, or other element to which it applies." ;
	.

gleif-base:hasTarget
	a
		owl:ObjectProperty ,
		owl:FunctionalProperty
		;
	rdfs:label "has target" ;
	rdfs:domain gleif-base:LegalEntityRelationship ;
	rdfs:isDefinedBy <https://www.gleif.org/ontology/Base/> ;
	rdfs:range gleif-base:Entity ;
	skos:definition "The entity that plays the target of the directed relationship." ;
	.

gleif-base:hasWebsite
	a owl:DatatypeProperty ;
	rdfs:label "has website" ;
	rdfs:isDefinedBy <https://www.gleif.org/ontology/Base/> ;
	rdfs:range xsd:anyURI ;
	skos:definition "A website associated with something, including but not limited to an organization." ;
	.

gleif-base:identifies
	a
		owl:ObjectProperty ,
		owl:FunctionalProperty
		;
	rdfs:label "identifies" ;
	rdfs:isDefinedBy <https://www.gleif.org/ontology/Base/> ;
	skos:definition "The relationship between an identifier and the thing it uniquely identifies." ;
	.

gleif-base:isManagedBy
	a owl:ObjectProperty ;
	rdfs:label "is managed by" ;
	rdfs:isDefinedBy <https://www.gleif.org/ontology/Base/> ;
	skos:definition "Relates something to another thing that has some role in directing its affairs." ;
	.

gleif-base:isQualifiedBy
	a owl:ObjectProperty ;
	rdfs:label "is qualified by" ;
	rdfs:domain gleif-base:LegalEntityRelationship ;
	rdfs:isDefinedBy <https://www.gleif.org/ontology/Base/> ;
	skos:definition "Any additional qualitative properties that help to categorize the relationship." ;
	.

gleif-base:isQuantifiedBy
	a owl:DatatypeProperty ;
	rdfs:label "is quantified by" ;
	rdfs:domain gleif-base:LegalEntityRelationship ;
	rdfs:isDefinedBy <https://www.gleif.org/ontology/Base/> ;
	rdfs:range xsd:decimal ;
	skos:definition "Any additional quantitative properties that help to categorize the relationship." ;
	.

gleif-base:isRegisteredIn
	a owl:ObjectProperty ;
	rdfs:label "is registered in" ;
	rdfs:isDefinedBy <https://www.gleif.org/ontology/Base/> ;
	rdfs:range gleif-base:Registry ;
	skos:definition "indicates the registry that something is registered in" ;
	.

gleif-base:records
	a
		owl:ObjectProperty ,
		owl:FunctionalProperty
		;
	rdfs:label "records" ;
	rdfs:domain gleif-base:RegistryEntry ;
	rdfs:isDefinedBy <https://www.gleif.org/ontology/Base/> ;
	skos:definition "The thing which the registry entry is a record of." ;
	.

[]
	a owl:AllDifferent ;
	owl:members (
		gleif-base:EntityExpirationReasonCorporateAction
		gleif-base:EntityExpirationReasonDissolved
		gleif-base:EntityExpirationReasonOther
	) ;
	.

[]
	a owl:AllDifferent ;
	owl:members (
		gleif-base:EntityStatusActive
		gleif-base:EntityStatusInactive
	) ;
	.

