# baseURI: https://www.gleif.org/ontology/EntityLegalForm/
# imports: http://www.omg.org/spec/LCC/Countries/CountryRepresentation/
# imports: https://www.gleif.org/ontology/Base/

@base <https://www.gleif.org/ontology/EntityLegalForm/> .
@prefix dct: <http://purl.org/dc/terms/> .
@prefix gleif-base: <https://www.gleif.org/ontology/Base/> .
@prefix gleif-elf: <https://www.gleif.org/ontology/EntityLegalForm/> .
@prefix lcc-cr: <http://www.omg.org/spec/LCC/Countries/CountryRepresentation/> .
@prefix owl: <http://www.w3.org/2002/07/owl#> .
@prefix rdf: <http://www.w3.org/1999/02/22-rdf-syntax-ns#> .
@prefix rdfs: <http://www.w3.org/2000/01/rdf-schema#> .
@prefix skos: <http://www.w3.org/2004/02/skos/core#> .
@prefix xsd: <http://www.w3.org/2001/XMLSchema#> .

<https://www.gleif.org/ontology/EntityLegalForm/>
	a owl:Ontology ;
	rdfs:label "GLEIF Entity Legal Form Ontology" ;
	dct:abstract "This ontology defines concepts for Entity Legal Forms" ;
	dct:license "http://opensource.org/licenses/MIT"^^xsd:anyURI ;
	dct:rights "Copyright (c) 2018 GLEIF" ;
	dct:source "https://www.gleif.org/en/about-lei/common-data-file-format/lei-cdf-format/lei-cdf-format-version-2-1"^^xsd:anyURI ;
	owl:imports
		<http://www.omg.org/spec/LCC/Countries/CountryRepresentation/> ,
		<https://www.gleif.org/ontology/Base/>
		;
	.

gleif-elf:ELFRegistrationStatus
	a owl:Class ;
	rdfs:subClassOf gleif-base:RegistrationStatus ;
	rdfs:label "ELF registration status" ;
	skos:definition "Status of an entry in a entity legal form registry that conforms to ISO 20275" ;
	.

gleif-elf:ELFRegistrationStatusActive
	a
		owl:NamedIndividual ,
		gleif-elf:ELFRegistrationStatus
		;
	rdfs:label "active" ;
	skos:definition "status indicating that the registration is active" ;
	gleif-base:hasTag "ACTV" ;
	.

gleif-elf:ELFRegistrationStatusInactive
	a
		owl:NamedIndividual ,
		gleif-elf:ELFRegistrationStatus
		;
	rdfs:label "inactive" ;
	skos:definition "status indicating that the registration is inactive" ;
	gleif-base:hasTag "INAC" ;
	.

gleif-elf:ELFregistry
	a gleif-base:Registry ;
	rdfs:label "GLEIF Entity Legal Forms List" ;
	skos:altLabel "ELF" ;
	gleif-base:hasWebsite "https://www.gleif.org/en/about-lei/code-lists/iso-20275-entity-legal-forms-code-list"^^xsd:anyURI ;
	gleif-base:isManagedBy gleif-base:GLEIF ;
	.

gleif-elf:EntityLegalForm
	a owl:Class ;
	rdfs:subClassOf
		[
			a owl:Restriction ;
			owl:onProperty gleif-base:hasLocalName ;
			owl:minCardinality "1"^^xsd:nonNegativeInteger ;
		] ,
		[
			a owl:Restriction ;
			owl:onProperty gleif-base:hasTransliteratedName ;
			owl:minCardinality "1"^^xsd:nonNegativeInteger ;
		] ,
		[
			a owl:Restriction ;
			owl:onProperty gleif-base:hasLocalAbbreviation ;
			owl:minQualifiedCardinality "0"^^xsd:nonNegativeInteger ;
			owl:onDataRange xsd:string ;
		] ,
		[
			a owl:Restriction ;
			owl:onProperty gleif-base:hasTransliteratedAbbreviation ;
			owl:minQualifiedCardinality "0"^^xsd:nonNegativeInteger ;
			owl:onDataRange xsd:string ;
		] ,
		[
			a owl:Restriction ;
			owl:onProperty gleif-base:hasLastModificationDate ;
			owl:onDataRange xsd:dateTime ;
			owl:qualifiedCardinality "1"^^xsd:nonNegativeInteger ;
		] ,
		[
			a owl:Restriction ;
			owl:onProperty gleif-base:hasCoverageArea ;
			owl:someValuesFrom lcc-cr:GeographicRegion ;
		] ,
		[
			a owl:Restriction ;
			owl:onProperty gleif-base:hasRegistrationStatus ;
			owl:someValuesFrom gleif-elf:ELFRegistrationStatus ;
		]
		;
	rdfs:label "entity legal form" ;
	skos:definition "The legal form of the entity, taken from the ISO Entity Legal Form (ELF) code list maintained by GLEIF. " ;
	.

gleif-elf:EntityLegalFormIdentifier
	a owl:Class ;
	rdfs:subClassOf
		gleif-base:Identifier ,
		[
			a owl:Restriction ;
			owl:onProperty gleif-base:identifies ;
			owl:onClass gleif-elf:EntityLegalForm ;
			owl:qualifiedCardinality "1"^^xsd:nonNegativeInteger ;
		]
		;
	rdfs:label "entity legal form identifier" ;
	owl:equivalentClass [
		a owl:Restriction ;
		owl:onProperty gleif-base:isRegisteredIn ;
		owl:hasValue gleif-elf:ELFregistry ;
	] ;
	skos:definition "A current code from the GLEIF-maintained list MUST be used. Values of the LegalFormEnum code list are maintained by GLEIF on behalf of ISO through the Entity Legal Form (ELF) as defined in ISO 20275." ;
	.

