# baseURI: https://www.gleif.org/ontology/Geocoding/
# imports: http://www.omg.org/spec/LCC/Countries/CountryRepresentation/
# imports: https://www.gleif.org/ontology/Base/

@base <https://www.gleif.org/ontology/Geocoding/> .
@prefix dct: <http://purl.org/dc/terms/> .
@prefix gleif-base: <https://www.gleif.org/ontology/Base/> .
@prefix gleif-geo: <https://www.gleif.org/ontology/Geocoding/> .
@prefix lcc-cr: <http://www.omg.org/spec/LCC/Countries/CountryRepresentation/> .
@prefix owl: <http://www.w3.org/2002/07/owl#> .
@prefix rdf: <http://www.w3.org/1999/02/22-rdf-syntax-ns#> .
@prefix rdfs: <http://www.w3.org/2000/01/rdf-schema#> .
@prefix skos: <http://www.w3.org/2004/02/skos/core#> .
@prefix wgs: <http://www.w3.org/2003/01/geo/wgs84_pos#> .
@prefix xml: <http://www.w3.org/XML/1998/namespace> .
@prefix xsd: <http://www.w3.org/2001/XMLSchema#> .

<https://www.gleif.org/ontology/Geocoding/>
	a owl:Ontology ;
	rdfs:label "GLEIF Geocoding Ontology" ;
	dct:abstract "This ontology defines concepts for Geocoding of addresses as used in the L1 Golden Copy Data. It makes use of the W3C WGS84 ontology for latitude and longitude." ;
	dct:contributor <https://plus.google.com/+PeteRivett> ;
	dct:issued "2019-02-01T00:00:00Z"^^xsd:dateTime ;
	dct:license "https://www.gleif.org/en/meta/lei-data-terms-of-use/"^^xsd:anyURI ;
	dct:publisher gleif-base:GLEIF ;
	dct:rights "Copyright (c) 2019 Global Legal Entity Identifier Foundation (GLEIF)" ;
	dct:rightsHolder gleif-base:GLEIF ;
	dct:source
		"https://developer.here.com/documentation/geocoder/topics/reading-geocoding-response.html"^^xsd:anyURI ,
		"https://www.gleif.org/en/lei-data/gleif-golden-copy"^^xsd:anyURI
		;
	dct:title "Global Legal Entity Identifier Foundation Geocoding Ontology "@en ;
	owl:imports
		<http://www.omg.org/spec/LCC/Countries/CountryRepresentation/> ,
		<https://www.gleif.org/ontology/Base/>
		;
	owl:versionIRI <https://www.gleif.org/ontology/Geocoding-v1.0/Geocoding/> ;
	.

gleif-geo:BoundingBox
	a owl:Class ;
	rdfs:subClassOf
		wgs:SpatialThing ,
		[
			a owl:Restriction ;
			owl:onProperty gleif-geo:bottomRight ;
			owl:onClass wgs:Point ;
			owl:qualifiedCardinality "1"^^xsd:nonNegativeInteger ;
		] ,
		[
			a owl:Restriction ;
			owl:onProperty gleif-geo:topLeft ;
			owl:onClass wgs:Point ;
			owl:qualifiedCardinality "1"^^xsd:nonNegativeInteger ;
		]
		;
	rdfs:label "bounding box" ;
	rdfs:isDefinedBy <https://www.gleif.org/ontology/Geocoding/> ;
	skos:definition "A geographic rectangular area bounded by its top left and bottom right points." ;
	.

gleif-geo:GeocodedAddress
	a owl:Class ;
	rdfs:subClassOf
		gleif-base:PhysicalAddress ,
		[
			a owl:Restriction ;
			owl:onProperty gleif-base:hasCity ;
			owl:cardinality "1" ;
		] ,
		[
			a owl:Restriction ;
			owl:onProperty gleif-geo:locationId ;
			owl:cardinality "1" ;
		] ,
		[
			a owl:Restriction ;
			owl:onProperty gleif-base:hasAddressNumber ;
			owl:maxCardinality "1" ;
		] ,
		[
			a owl:Restriction ;
			owl:onProperty gleif-base:hasPostalCode ;
			owl:maxCardinality "1" ;
		] ,
		[
			a owl:Restriction ;
			owl:onProperty gleif-geo:formattedAddressText ;
			owl:maxCardinality "1" ;
		] ,
		[
			a owl:Restriction ;
			owl:onProperty gleif-geo:hasDistrict ;
			owl:maxCardinality "1" ;
		] ,
		[
			a owl:Restriction ;
			owl:onProperty gleif-geo:hasRegionText ;
			owl:maxCardinality "1" ;
		] ,
		[
			a owl:Restriction ;
			owl:onProperty gleif-geo:hasStreet ;
			owl:maxCardinality "1" ;
		] ,
		[
			a owl:Restriction ;
			owl:onProperty gleif-geo:originalAddressText ;
			owl:minCardinality "0" ;
		] ,
		[
			a owl:Restriction ;
			owl:onProperty gleif-geo:originalAddress ;
			owl:onClass gleif-base:PhysicalAddress ;
			owl:minQualifiedCardinality "0" ;
		] ,
		[
			a owl:Restriction ;
			owl:onProperty gleif-base:hasCountry ;
			owl:onClass lcc-cr:Country ;
			owl:qualifiedCardinality "1" ;
		] ,
		[
			a owl:Restriction ;
			owl:onProperty gleif-geo:hasBoundingBox ;
			owl:onClass gleif-geo:BoundingBox ;
			owl:qualifiedCardinality "1" ;
		] ,
		[
			a owl:Restriction ;
			owl:onProperty gleif-geo:matchType ;
			owl:onClass gleif-geo:MatchType ;
			owl:qualifiedCardinality "1" ;
		] ,
		[
			a owl:Restriction ;
			owl:onProperty gleif-geo:matchDate ;
			owl:onDataRange xsd:dateTime ;
			owl:qualifiedCardinality "1" ;
		] ,
		[
			a owl:Restriction ;
			owl:onProperty gleif-geo:relevance ;
			owl:onDataRange xsd:decimal ;
			owl:qualifiedCardinality "1" ;
		]
		;
	rdfs:label "geocoded address"@en ;
	rdfs:isDefinedBy <https://www.gleif.org/ontology/Geocoding/> ;
	skos:definition "A geocoded address, derived from a physical address, with latitude and longitude information." ;
	.

gleif-geo:MatchType
	a owl:Class ;
	rdfs:label "match type" ;
	rdfs:isDefinedBy <https://www.gleif.org/ontology/Geocoding/> ;
	owl:oneOf (
		gleif-geo:MatchTypePointAddress
		gleif-geo:MatchTypeInterpolated
	) ;
	skos:definition "Quality of the location match, either pointAddress or interpolated." ;
	.

gleif-geo:MatchTypeInterpolated
	a gleif-geo:MatchType ;
	rdfs:label "match type interpolated" ;
	rdfs:isDefinedBy <https://www.gleif.org/ontology/Geocoding/> ;
	skos:definition "The location was interpolated from known locations of adjacent addresses." ;
	gleif-base:hasTag "interpolated" ;
	.

gleif-geo:MatchTypePointAddress
	a gleif-geo:MatchType ;
	rdfs:label "match type point address" ;
	rdfs:isDefinedBy <https://www.gleif.org/ontology/Geocoding/> ;
	skos:definition "The location matches the specific address." ;
	gleif-base:hasTag "pointAddress" ;
	.

gleif-geo:bottomRight
	a owl:ObjectProperty ;
	rdfs:label "bottom right" ;
	rdfs:domain gleif-geo:BoundingBox ;
	rdfs:isDefinedBy <https://www.gleif.org/ontology/Geocoding/> ;
	rdfs:range wgs:Point ;
	skos:definition "The bottom right point of a bounding box." ;
	.

gleif-geo:formattedAddressText
	a owl:DatatypeProperty ;
	rdfs:label "formatted address text" ;
	rdfs:domain gleif-geo:GeocodedAddress ;
	rdfs:isDefinedBy <https://www.gleif.org/ontology/Geocoding/> ;
	skos:definition "An aggregated textual representation of the the fields produced by the geocoding as a comma-separated list of fields." ;
	.

gleif-geo:hasBoundingBox
	a owl:ObjectProperty ;
	rdfs:label "has bounding box" ;
	rdfs:domain gleif-geo:GeocodedAddress ;
	rdfs:isDefinedBy <https://www.gleif.org/ontology/Geocoding/> ;
	rdfs:range gleif-geo:BoundingBox ;
	skos:definition "The geographic area represented by the address." ;
	.

gleif-geo:hasDistrict
	a owl:DatatypeProperty ;
	rdfs:label "has district" ;
	rdfs:domain gleif-geo:GeocodedAddress ;
	rdfs:isDefinedBy <https://www.gleif.org/ontology/Geocoding/> ;
	skos:definition "A textual representation of the district." ;
	.

gleif-geo:hasRegionText
	a owl:DatatypeProperty ;
	rdfs:label "has region text" ;
	rdfs:domain gleif-geo:GeocodedAddress ;
	rdfs:isDefinedBy <https://www.gleif.org/ontology/Geocoding/> ;
	skos:altLabel "has state text" ;
	skos:definition "A textual representation of the state or region." ;
	skos:prefLabel "has region text" ;
	.

gleif-geo:hasStreet
	a owl:DatatypeProperty ;
	rdfs:label "has street" ;
	rdfs:domain gleif-geo:GeocodedAddress ;
	rdfs:isDefinedBy <https://www.gleif.org/ontology/Geocoding/> ;
	skos:definition "The name of a street, as opposed to a house within it." ;
	.

gleif-geo:locationId
	a owl:DatatypeProperty ;
	rdfs:subPropertyOf gleif-base:hasTag ;
	rdfs:label "location ID" ;
	rdfs:domain gleif-geo:GeocodedAddress ;
	rdfs:isDefinedBy <https://www.gleif.org/ontology/Geocoding/> ;
	skos:definition "A unique identifier representing a hash of the location." ;
	.

gleif-geo:matchDate
	a owl:DatatypeProperty ;
	rdfs:label "has end"@en ;
	rdfs:domain gleif-geo:GeocodedAddress ;
	rdfs:isDefinedBy <https://www.gleif.org/ontology/Geocoding/> ;
	rdfs:range xsd:dateTime ;
	skos:definition "The date of the geocoding from the original address." ;
	.

gleif-geo:matchLevel
	a owl:AnnotationProperty ;
	rdfs:label "match level" ;
	rdfs:domain gleif-geo:GeocodedAddress ;
	rdfs:isDefinedBy <https://www.gleif.org/ontology/Geocoding/> ;
	rdfs:range owl:DatatypeProperty ;
	skos:definition "The most detailed address field that the geocoding was able to provide." ;
	.

gleif-geo:matchType
	a owl:ObjectProperty ;
	rdfs:label "match type" ;
	rdfs:domain gleif-geo:GeocodedAddress ;
	rdfs:isDefinedBy <https://www.gleif.org/ontology/Geocoding/> ;
	rdfs:range gleif-geo:MatchType ;
	skos:definition "Quality of the location match, either pointAddress or interpolated." ;
	.

gleif-geo:originalAddress
	a owl:ObjectProperty ;
	rdfs:label "original address" ;
	rdfs:domain gleif-geo:GeocodedAddress ;
	rdfs:isDefinedBy <https://www.gleif.org/ontology/Geocoding/> ;
	rdfs:range gleif-base:PhysicalAddress ;
	skos:definition "The original address(es) from which the geocoding was derived." ;
	.

gleif-geo:originalAddressText
	a owl:DatatypeProperty ;
	rdfs:label "original address text" ;
	rdfs:domain gleif-geo:GeocodedAddress ;
	rdfs:isDefinedBy <https://www.gleif.org/ontology/Geocoding/> ;
	skos:definition "An aggregated textual representation of the original address(es) from which the geocoding was derived, as a comma-separated list of fields with null where the field did not have a value." ;
	.

gleif-geo:relevance
	a owl:DatatypeProperty ;
	rdfs:label "bottom right" ;
	rdfs:domain gleif-geo:GeocodedAddress ;
	rdfs:isDefinedBy <https://www.gleif.org/ontology/Geocoding/> ;
	rdfs:range xsd:decimal ;
	skos:definition "A value from 0 to 1 representing the percentage of the input that matched the returned address. 1 means that all input tokens were matched." ;
	.

gleif-geo:topLeft
	a owl:ObjectProperty ;
	rdfs:label "top left" ;
	rdfs:domain gleif-geo:BoundingBox ;
	rdfs:isDefinedBy <https://www.gleif.org/ontology/Geocoding/> ;
	rdfs:range wgs:Point ;
	skos:definition "The top left point of a bounding box." ;
	.

[]
	a owl:AllDifferent ;
	owl:members (
		gleif-geo:MatchTypePointAddress
		gleif-geo:MatchTypeInterpolated
	) ;
	.

