# baseURI: https://www.gleif.org/ontology/L1/
# imports: https://www.gleif.org/ontology/Base/
# imports: https://www.gleif.org/ontology/EntityLegalForm/
# imports: https://www.gleif.org/ontology/RegistrationAuthority/

@base <https://www.gleif.org/ontology/L1/> .
@prefix dct: <http://purl.org/dc/terms/> .
@prefix gleif-L1: <https://www.gleif.org/ontology/L1/> .
@prefix gleif-base: <https://www.gleif.org/ontology/Base/> .
@prefix gleif-elf: <https://www.gleif.org/ontology/EntityLegalForm/> .
@prefix gleif-ra: <https://www.gleif.org/ontology/RegistrationAuthority/> .
@prefix lcc-cr: <https://www.omg.org/spec/LCC/Countries/CountryRepresentation/> .
@prefix owl: <http://www.w3.org/2002/07/owl#> .
@prefix rdf: <http://www.w3.org/1999/02/22-rdf-syntax-ns#> .
@prefix rdfs: <http://www.w3.org/2000/01/rdf-schema#> .
@prefix skos: <http://www.w3.org/2004/02/skos/core#> .
@prefix vann: <http://purl.org/vocab/vann/> .
@prefix voaf: <http://purl.org/vocommons/voaf#> .
@prefix xsd: <http://www.w3.org/2001/XMLSchema#> .

<https://www.gleif.org/ontology/L1/>
	a
		voaf:Vocabulary ,
		owl:Ontology
		;
	rdfs:label "GLEIF L1 Ontology" ;
	dct:abstract """Ontology for legal entity identifier registration. It was designed for Global Legal Entity Identifier Foundation (GLEIF) Level 1 data corresponding to the Common Data Format version 2.1. It covers key reference data for a legal entity identifiable with an LEI. The ISO 17442 standard developed by the International Organization for Standardization defines a set of attributes or LEI reference data that comprises the most essential elements of identification. It specifies the minimum reference data, which must be supplied for each LEI:
    The official name of the legal entity as recorded in the official registers.
    The registered address of that legal entity.
    The country of formation.
    The codes for the representation of names of countries and their subdivisions.
    The date of the first LEI assignment; the date of last update of the LEI information; and the date of expiry, if applicable."""@en ;
	dct:contributor
		<http://purl.org/bryon> ,
		<http://www.workingontologist.com> ,
		<https://www.linkedin.com/in/peterivett/>
		;
	dct:creator gleif-base:GLEIF ;
	dct:issued "2022-01-06T00:00:00Z"^^xsd:dateTime ;
	dct:license "https://www.gleif.org/en/meta/lei-data-terms-of-use/"^^xsd:anyURI ;
	dct:rights "Copyright (c) 2019-2022 Global Legal Entity Identifier Foundation (GLEIF)" ;
	dct:rights "Copyright (c) 2021-2022 agnos.ai UK Ltd." ;
	dct:rightsHolder gleif-base:GLEIF ;
	dct:source "https://www.gleif.org/en/about-lei/common-data-file-format/lei-cdf-format/lei-cdf-format-version-3-1"^^xsd:anyURI ;
	dct:title "Global Legal Entity Identifier Foundation Level 1 Ontology - Who Is Who"@en ;
	vann:preferredNamespacePrefix "gleif-L1" ;
	vann:preferredNamespaceUri "https://www.gleif.org/ontology/L1/" ;
	owl:imports
		<https://www.gleif.org/ontology/Base/> ,
		<https://www.gleif.org/ontology/EntityLegalForm/> ,
		<https://www.gleif.org/ontology/RegistrationAuthority/>
		;
	owl:versionIRI <https://www.gleif.org/ontology/L1-v1.1/L1/> ;
	skos:changeNote "Version 1.0.1 made a minor fix to 2 restrictions on LegalEntityRelationship"@en ;
	skos:changeNote "Version 1.1 reflects GLEIF LEI-CDF version 3.1, and removes wrong superclass of ValidationSourceKind"@en ;
	.

gleif-L1:Branch
	a owl:Class ;
	rdfs:subClassOf gleif-L1:RegisteredEntity ;
	rdfs:label "branch" ;
	rdfs:isDefinedBy <https://www.gleif.org/ontology/L1/> ;
	skos:definition "The entity is a branch of another legal entity." ;
	.

gleif-L1:BusinessRegistryIdentifier
	a owl:Class ;
	rdfs:subClassOf
		gleif-base:RegistryIdentifier ,
		[
			a owl:Restriction ;
			owl:onProperty gleif-L1:hasOtherAuthority ;
			owl:maxCardinality "1"^^xsd:nonNegativeInteger ;
		] ,
		[
			a owl:Restriction ;
			owl:onProperty gleif-L1:hasRegisteredAuthority ;
			owl:onClass gleif-ra:BusinessRegistry ;
			owl:maxQualifiedCardinality "1"^^xsd:nonNegativeInteger ;
		] ,
		[
			a owl:Restriction ;
			owl:onProperty gleif-base:identifies ;
			owl:onClass gleif-L1:RegisteredEntity ;
			owl:qualifiedCardinality "1"^^xsd:nonNegativeInteger ;
		] ,
		[
			a owl:Restriction ;
			owl:onProperty gleif-L1:hasEntityID ;
			owl:onDataRange xsd:string ;
			owl:qualifiedCardinality "1"^^xsd:nonNegativeInteger ;
		] ,
		[
			owl:intersectionOf (
				[
					a owl:Class ;
					owl:unionOf (
						[
							a owl:Restriction ;
							owl:onProperty gleif-L1:hasRegisteredAuthority ;
							owl:onClass gleif-ra:BusinessRegistry ;
							owl:qualifiedCardinality "1"^^xsd:nonNegativeInteger ;
						]
						[
							a owl:Restriction ;
							owl:onProperty gleif-L1:hasOtherAuthority ;
							owl:cardinality "1"^^xsd:nonNegativeInteger ;
						]
					) ;
				]
				[
					a owl:Class ;
					owl:complementOf [
						a owl:Class ;
						owl:intersectionOf (
							[
								a owl:Restriction ;
								owl:onProperty gleif-L1:hasRegisteredAuthority ;
								owl:someValuesFrom gleif-ra:BusinessRegistry ;
							]
							[
								a owl:Restriction ;
								owl:onProperty gleif-L1:hasOtherAuthority ;
								owl:minCardinality "1"^^xsd:nonNegativeInteger ;
							]
						) ;
					] ;
				]
			) ;
		]
		;
	rdfs:label "business registry identifier" ;
	rdfs:isDefinedBy <https://www.gleif.org/ontology/L1/> ;
	skos:definition "The legal entity is a branch of another legal entity." ;
	.

gleif-L1:CentralGovernment
	a owl:Class ;
	rdfs:subClassOf gleif-L1:ResidentGovernmentEntity ;
	rdfs:label "central government" ;
	rdfs:isDefinedBy <https://www.gleif.org/ontology/L1/> ;
	skos:altLabel
		"central government entity" 
		;
	skos:definition "The legal entity is in a central government subsector which consists of the institutional units plus non-profit institutions (NPI) controlled by the central government institutions." ;
	skos:prefLabel "central government" ;
	.

gleif-L1:Fund
	a owl:Class ;
	rdfs:subClassOf gleif-L1:RegisteredEntity ;
	rdfs:label "fund" ;
	rdfs:isDefinedBy <https://www.gleif.org/ontology/L1/> ;
	skos:definition "The legal entity is an investment fund defined as a collective investment scheme (or pooled investment) beneficially owned by multiple investors and managed on behalf of those investors by an asset manager or by the fund itself." ;
	.

gleif-L1:FundFamily
	a owl:Class ;
	rdfs:subClassOf gleif-L1:LegalEntity ;
	rdfs:label "fund family" ;
	rdfs:isDefinedBy <https://www.gleif.org/ontology/L1/> ;
	skos:definition "The entity that is the manager of one or more funds." ;
	owl:deprecated "true"^^xsd:boolean ;
	.

gleif-L1:GeneralEntity
	a owl:Class ;
	rdfs:subClassOf gleif-L1:RegisteredEntity ;
	rdfs:label "general entity" ;
	rdfs:isDefinedBy <https://www.gleif.org/ontology/L1/> ;
	skos:definition "The legal entity is a general legal entity." ;
	.

gleif-L1:GlobalLegalEntityIdentifierSystem
	a gleif-base:Registry ;
	rdfs:label "Global Legal Entity Identifier System" ;
	rdfs:isDefinedBy <https://www.gleif.org/ontology/L1/> ;
	skos:altLabel "GLEIS" ;
	skos:definition "The global repository of LEIs and reference data." ;
	skos:prefLabel "Global Legal Entity Identifier System" ;
	gleif-base:hasWebsite "https://www.gleif.org/en/about-lei/gleif-management-of-the-global-lei-system"^^xsd:anyURI ;
	gleif-base:isManagedBy gleif-base:GLEIF ;
	.

gleif-L1:InternationalOrganization
	a owl:Class ;
	rdfs:subClassOf gleif-L1:LegalEntity ;
	rdfs:label "international organization" ;
	rdfs:isDefinedBy <https://www.gleif.org/ontology/L1/> ;
	skos:altLabel
		"intergovernmental organization" 
		;
	skos:definition "The legal entity is a non-resident unit created by international agreements or other arrangements for the provision of non-market services or financial intermediation at the international level." ;
	skos:prefLabel "international organization" ;
	.

gleif-L1:LEI
	a
		owl:DatatypeProperty ,
		owl:FunctionalProperty
		;
	rdfs:subPropertyOf gleif-base:hasTag ;
	rdfs:label "LEI" ;
	rdfs:isDefinedBy <https://www.gleif.org/ontology/L1/> ;
	rdfs:range xsd:string ;
	skos:altLabel "has LEI string" ;
	skos:definition "The ISO 17442 compatible identifier for the legal entity recorded." ;
	skos:prefLabel "LEI" ;
	.

gleif-L1:LegalEntity
	a owl:Class ;
	rdfs:subClassOf
		gleif-base:LegalPerson ,
		gleif-L1:RegisteredEntity
		;
	rdfs:label "legal entity" ;
	rdfs:isDefinedBy <https://www.gleif.org/ontology/L1/> ;
	skos:definition "LEI-registered entities that are legally or financially responsible for the performance of financial transactions or have the legal right in their jurisdiction to enter independently into legal contracts, regardless of whether they are incorporated or constituted in some other way (e.g. trust, partnership, contractual). It excludes natural persons, but includes governmental organizations and supranationals." ;
	.

gleif-L1:LegalEntityEvent
	a owl:Class ;
	rdfs:subClassOf
		gleif-base:Event ,
		[
			a owl:Restriction ;
			owl:onProperty gleif-base:hasEventKind ;
			owl:onClass [
				a owl:Class ;
				owl:oneOf (
					gleif-L1:LegalEntityEventKindChangeLegalName
					gleif-L1:LegalEntityEventKindChangeOtherNames
					gleif-L1:LegalEntityEventKindChangeLegalAddress
					gleif-L1:LegalEntityEventKindChangeHQAddress
					gleif-L1:LegalEntityEventKindChangeLegalForm
					gleif-L1:LegalEntityEventKindDemerger
					gleif-L1:LegalEntityEventKindSpinoff
					gleif-L1:LegalEntityEventKindAbsorption
					gleif-L1:LegalEntityEventKindAcquisitionBranch
					gleif-L1:LegalEntityEventKindTransformationBranchToSubsidiary
					gleif-L1:LegalEntityEventKindTransformationSubsidiaryToBranch
					gleif-L1:LegalEntityEventKindTransformationUmbrellaToStandalone
					gleif-L1:LegalEntityEventKindBreakup
					gleif-L1:LegalEntityEventKindMergersAndAcquisitions
					gleif-L1:LegalEntityEventKindBankruptcy
					gleif-L1:LegalEntityEventKindLiquidation
					gleif-L1:LegalEntityEventKindVoluntaryArrangement
					gleif-L1:LegalEntityEventKindInsolvency
					gleif-L1:LegalEntityEventKindDissolution
				) ;
			] ;
			owl:cardinality "1"^^xsd:nonNegativeInteger ;
		] ,
		[
			a owl:Restriction ;
			owl:onProperty gleif-base:hasEventStatus ;
			owl:onClass [
				a owl:Class ;
				owl:oneOf (
					gleif-L1:LegalEntityEventStatusInProgress
					gleif-L1:LegalEntityEventStatusWithdrawnCancelled
					gleif-L1:LegalEntityEventStatusCompleted
				) ;
			] ;
			owl:cardinality "1"^^xsd:nonNegativeInteger ;
		] ,[
			a owl:Restriction ;
			owl:onProperty gleif-base:hasEffectiveDate ;
			owl:maxQualifiedCardinality "0"^^xsd:nonNegativeInteger ;
			owl:onDataRange xsd:dateTime ;
		] ,
		[
			a owl:Restriction ;
			owl:onProperty gleif-base:hasRecordedDate ;
			owl:maxQualifiedCardinality "1"^^xsd:nonNegativeInteger ;
			owl:onDataRange xsd:dateTime ;
		] ,
		[
			a owl:Restriction ;
			owl:onProperty gleif-base:hasValidationDocuments ;
			owl:onClass gleif-base:ValidationDocumentsKind ;
			owl:minQualifiedCardinality "1"^^xsd:nonNegativeInteger ;
		] ,
		[
			a owl:Restriction ;
			owl:onProperty gleif-base:hasValidationReference ;
			owl:onDataRange xsd:string ;
			owl:minQualifiedCardinality "0"^^xsd:nonNegativeInteger ;
		]
	;
	rdfs:label "legal entity event" ;
	rdfs:isDefinedBy <https://www.gleif.org/ontology/L1/> ;
	skos:definition "A single event specified by the LEI ROC in the life of a legal entity that would impact the Reference Data in the Global LEI System."
.

gleif-L1:LegalEntityEventGroup
	a owl:Class ;
	rdfs:subClassOf
		[
			a owl:Restriction ;
			owl:onProperty gleif-L1:hasGroupedEvent ;
			owl:someValuesFrom gleif-L1:LegalEntityEvent ;
		] ,
		[
			a owl:Restriction ;
			owl:onProperty gleif-L1:hasLegalEntityEventGroupKind ;
			owl:onClass [
				a owl:Class ;
				owl:oneOf (
					gleif-L1:LegalEntityEventGroupKindReverseTakeover
					gleif-L1:LegalEntityEventGroupKindChangeLegalFormAndName
					gleif-L1:LegalEntityEventGroupKindComplexChangeLegalForm
				) ;
			] ;
			owl:cardinality "1"^^xsd:nonNegativeInteger ;
		] ;
	rdfs:label "legal entity event group" ;
	rdfs:isDefinedBy <https://www.gleif.org/ontology/L1/> ;
	skos:definition "A complex event." ;
.

gleif-L1:LegalEntitySequencedEvent 
	a owl:Class ;
	rdfs:subClassOf 
			[
			a owl:Restriction ;
			owl:onProperty gleif-L1:hasGroupedEvent ;
			owl:onClass gleif-L1:LegalEntityEvent ;
			owl:cardinality "1"^^xsd:nonNegativeInteger ;
		] ,
			[
			a owl:Restriction ;
			owl:onProperty gleif-L1:hasSequenceNumber ;
			owl:onDataRange xsd:positiveInteger ;
			owl:cardinality "1"^^xsd:nonNegativeInteger ;
		] 
 	;
	rdfs:label "legal entity sequenced event" ;
	rdfs:isDefinedBy <https://www.gleif.org/ontology/L1/> ;
	skos:definition "An event in a group where the sequence is significant."
.

gleif-L1:LegalEntityEventKind
	a owl:Class ;
	rdfs:subClassOf gleif-base:EventKind ;
	rdfs:label "legal entity event kind" ;
	rdfs:isDefinedBy <https://www.gleif.org/ontology/L1/> ;
	skos:definition "A single event specified by the LEI ROC in the life of a legal entity that would impact the Reference Data in the Global LEI System."
.

gleif-L1:LegalEntityEventKindChangeLegalName
	a
		owl:NamedIndividual ,
		gleif-L1:LegalEntityEventKind ;
	rdfs:label "change legal name" ;
	rdfs:isDefinedBy <https://www.gleif.org/ontology/L1/> ;
	skos:definition "Change in the legal name of the legal entity." ;
	gleif-base:hasTag "CHANGE_LEGAL_NAME" ;
.

gleif-L1:LegalEntityEventKindChangeOtherNames
	a
		owl:NamedIndividual ,
		gleif-L1:LegalEntityEventKind ;
	rdfs:label "change other names" ;
	rdfs:isDefinedBy <https://www.gleif.org/ontology/L1/> ;
	skos:definition "Change in the trade- or doing business name of the legal entity." ;
	gleif-base:hasTag "CHANGE_OTHER_NAMES" ;
.

gleif-L1:LegalEntityEventKindChangeLegalAddress
	a
		owl:NamedIndividual ,
		gleif-L1:LegalEntityEventKind ;
	rdfs:label "change legal address" ;
	rdfs:isDefinedBy <https://www.gleif.org/ontology/L1/> ;
	skos:definition "Change in the legal address of the legal entity." ;
	gleif-base:hasTag "CHANGE_LEGAL_ADDRESS" ;
.

gleif-L1:LegalEntityEventKindChangeHQAddress
	a
		owl:NamedIndividual ,
		gleif-L1:LegalEntityEventKind ;
	rdfs:label "change HQ address" ;
	rdfs:isDefinedBy <https://www.gleif.org/ontology/L1/> ;
	skos:definition "Change in the headquarters address of the legal entity." ;
	gleif-base:hasTag "CHANGE_HQ_ADDRESS" ;
.

gleif-L1:LegalEntityEventKindChangeLegalForm
	a
		owl:NamedIndividual ,
		gleif-L1:LegalEntityEventKind ;
	rdfs:label "change legal form" ;
	rdfs:isDefinedBy <https://www.gleif.org/ontology/L1/> ;
	skos:definition "Change in the legal form of the legal entity." ;
	gleif-base:hasTag "CHANGE_LEGAL_FORM" ;
.

gleif-L1:LegalEntityEventKindDemerger
	a
		owl:NamedIndividual ,
		gleif-L1:LegalEntityEventKind ;
	rdfs:label "demerger" ;
	rdfs:isDefinedBy <https://www.gleif.org/ontology/L1/> ;
	skos:definition "Distribution of securities issued by another legal entity. The distributed securities may either be of a newly created or of an existing legal entity. For example, spin-off, demerger, unbundling, divestment." ;
	gleif-base:hasTag "DEMERGER" ;
.

gleif-L1:LegalEntityEventKindSpinoff
	a
		owl:NamedIndividual ,
		gleif-L1:LegalEntityEventKind ;
	rdfs:label "spinoff" ;
	rdfs:isDefinedBy <https://www.gleif.org/ontology/L1/> ;
	skos:definition "A special case of demerger where the shareholders of the original entity are compensated for the value loss of the original entity via shares of the new entity or via dividend." ;
	gleif-base:hasTag "SPINOFF" ;
.

gleif-L1:LegalEntityEventKindAbsorption
	a
		owl:NamedIndividual ,
		gleif-L1:LegalEntityEventKind ;
	rdfs:label "absorption" ;
	rdfs:isDefinedBy <https://www.gleif.org/ontology/L1/> ;
	skos:definition "Absorption is a form of merger where there is a combination of two or more companies into an 'existing company'. In the case of absorption, only one company survives and all others lose their identity." ;
	gleif-base:hasTag "ABSORPTION" ;
.

gleif-L1:LegalEntityEventKindAcquisitionBranch
	a
		owl:NamedIndividual ,
		gleif-L1:LegalEntityEventKind ;
	rdfs:label "acquisition branch" ;
	rdfs:isDefinedBy <https://www.gleif.org/ontology/L1/> ;
	skos:definition "The acquiring legal entity purchases an international branch entity." ;
	gleif-base:hasTag "ACQUISITION_BRANCH" ;
.

gleif-L1:LegalEntityEventKindTransformationBranchToSubsidiary
	a
		owl:NamedIndividual ,
		gleif-L1:LegalEntityEventKind ;
	rdfs:label "transformation branch to subsidiary" ;
	rdfs:isDefinedBy <https://www.gleif.org/ontology/L1/> ;
	skos:definition "The transfer of all of the assets and liabilities of an International Branch to the new subsidiary entity in exchange for the transfer of securities representing the capital of the subsidiary entity receiving the transfer." ;
	gleif-base:hasTag "TRANSFORMATION_BRANCH_TO_SUBSIDIARY" ;
.

gleif-L1:LegalEntityEventKindTransformationSubsidiaryToBranch
	a
		owl:NamedIndividual ,
		gleif-L1:LegalEntityEventKind ;
	rdfs:label "transformation subsidiary to branch" ;
	rdfs:isDefinedBy <https://www.gleif.org/ontology/L1/> ;
	skos:definition "The transfer of all of the assets and liabilities of a subsidiary to an International Branch entity in exchange for the transfer of securities representing the capital of the International Branch entity receiving the transfer." ;
	gleif-base:hasTag "TRANSFORMATION_SUBSIDIARY_TO_BRANCH" ;
.

gleif-L1:LegalEntityEventKindTransformationUmbrellaToStandalone
	a
		owl:NamedIndividual ,
		gleif-L1:LegalEntityEventKind ;
	rdfs:label "transformation umbrella to standalone" ;
	rdfs:isDefinedBy <https://www.gleif.org/ontology/L1/> ;
	skos:definition "Change in legal form from a Fund legal entity structure with one or more than one sub-funds/compartments to a Fund legal entity structure without sub-funds/compartments." ;
	gleif-base:hasTag "TRANSFORMATION_UMBRELLA_TO_STANDALONE" ;
.

gleif-L1:LegalEntityEventKindBreakup
	a
		owl:NamedIndividual ,
		gleif-L1:LegalEntityEventKind ;
	rdfs:label "break-up" ;
	rdfs:isDefinedBy <https://www.gleif.org/ontology/L1/> ;
	skos:definition "A break-up is a corporate action in which a single company splits into two or more independent, separately-run companies.  Regulators also can mandate break-ups of companies for anti-trust reasons." ;
	gleif-base:hasTag "BREAKUP" ;
.

gleif-L1:LegalEntityEventKindMergersAndAcquisitions
	a
		owl:NamedIndividual ,
		gleif-L1:LegalEntityEventKind ;
	rdfs:label "mergers and acquisitions" ;
	rdfs:isDefinedBy <https://www.gleif.org/ontology/L1/> ;
	skos:definition "The consolidation of Legal Entities or assets through various types of financial transactions, including mergers, acquisitions, consolidations, tender offers, purchase of assets and management acquisitions." ;
	gleif-base:hasTag "MERGERS_AND_ACQUISITIONS" ;
.

gleif-L1:LegalEntityEventKindBankruptcy
	a
		owl:NamedIndividual ,
		gleif-L1:LegalEntityEventKind ;
	rdfs:label "bankruptcy" ;
	rdfs:isDefinedBy <https://www.gleif.org/ontology/L1/> ;
	skos:definition "Legal status of a legal entity unable to pay creditors. Bankruptcy usually involves a formal court ruling. Securities may become valueless (event completed)." ;
	gleif-base:hasTag "BANKRUPTCY" ;
.

gleif-L1:LegalEntityEventKindLiquidation
	a
		owl:NamedIndividual ,
		gleif-L1:LegalEntityEventKind ;
	rdfs:label "liquidation" ;
	rdfs:isDefinedBy <https://www.gleif.org/ontology/L1/> ;
	skos:definition "Distribution of cash, assets or both of a legal entity. Debt may be paid in order of priority based on preferred claims to assets specified by the security (event completed)." ;
	gleif-base:hasTag "LIQUIDATION" ;
.

gleif-L1:LegalEntityEventKindVoluntaryArrangement
	a
		owl:NamedIndividual ,
		gleif-L1:LegalEntityEventKind ;
	rdfs:label "voluntary arrangement" ;
	rdfs:isDefinedBy <https://www.gleif.org/ontology/L1/> ;
	skos:definition "A procedure that allows a legal entity to settle debts by paying only a proportion of the amount that it owes to creditors or to come to some other arrangement with its creditors over the payment of its debts (event completed)." ;
	gleif-base:hasTag "VOLUNTARY_ARRANGEMENT" ;
.

gleif-L1:LegalEntityEventKindInsolvency
	a
		owl:NamedIndividual ,
		gleif-L1:LegalEntityEventKind ;
	rdfs:label "insolvency" ;
	rdfs:isDefinedBy <https://www.gleif.org/ontology/L1/> ;
	skos:definition "The entry of a decree or order by a court or agency or supervisory authority having jurisdiction in the premises the appointment of a trustee-in-bankruptcy or similar official for such party in any insolvency, readjustment of debt, marshalling of assets and liabilities, or similar proceedings, or for the winding up or liquidation of their respective affairs (event completed)." ;
	gleif-base:hasTag "INSOLVENCY" ;
.

gleif-L1:LegalEntityEventKindDissolution
	a
		owl:NamedIndividual ,
		gleif-L1:LegalEntityEventKind ;
	rdfs:label "dissolution" ;
	rdfs:isDefinedBy <https://www.gleif.org/ontology/L1/> ;
	skos:definition "(i) A voluntary termination of operations, (ii) a general assignment for the benefit of the legal entityâ€™s creditors or (iii) any other liquidation, dissolution or winding up of the legal entity (excluding a Liquidity Event), whether voluntary or involuntary (event completed)." ;
	gleif-base:hasTag "DISSOLUTION" ;
.

gleif-L1:LegalEntityEventGroupKind
	a owl:Class ;
	rdfs:label "legal entity event group kind" ;
	rdfs:isDefinedBy <https://www.gleif.org/ontology/L1/> ;
	skos:definition "A complex event specified by the LEI ROC in the life of a legal entity that would impact the Reference Data in the Global LEI System."
.

gleif-L1:LegalEntityEventGroupKindReverseTakeover
	a
		owl:NamedIndividual ,
		gleif-L1:LegalEntityEventGroupKind ;
	rdfs:label "reverse takeover" ;
	rdfs:isDefinedBy <https://www.gleif.org/ontology/L1/> ;
	skos:definition "A reverse takeover event" ;
	gleif-base:hasTag "REVERSE_TAKEOVER" ;
.

gleif-L1:LegalEntityEventGroupKindChangeLegalFormAndName
	a
		owl:NamedIndividual ,
		gleif-L1:LegalEntityEventGroupKind ;
	rdfs:label "change legal form and name" ;
	rdfs:isDefinedBy <https://www.gleif.org/ontology/L1/> ;
	skos:definition "Legal entity event including change of the legal name triggered by change of the legal form." ;
	gleif-base:hasTag "CHANGE_LEGAL_FORM_AND_NAME" ;
.

gleif-L1:LegalEntityEventGroupKindComplexChangeLegalForm
	a
		owl:NamedIndividual ,
		gleif-L1:LegalEntityEventGroupKind ;
	rdfs:label "complex change legal form" ;
	rdfs:isDefinedBy <https://www.gleif.org/ontology/L1/> ;
	skos:definition "Legal entity event including change of the legal entity status triggered by change of the legal form." ;
	gleif-base:hasTag "COMPLEX_CHANGE_LEGAL_FORM" ;
.

gleif-L1:LegalEntityEventStatus
	a owl:Class ;
	rdfs:subClassOf gleif-base:EventStatus ;
	rdfs:label "legal entity event status" ;
	rdfs:isDefinedBy <https://www.gleif.org/ontology/L1/> ;
	skos:definition "The status of the legal entity event with regard to event timeline."
.

gleif-L1:LegalEntityEventStatusInProgress
	a
		owl:NamedIndividual ,
		gleif-L1:LegalEntityEventStatus ;
	rdfs:label "in progress" ;
	rdfs:isDefinedBy <https://www.gleif.org/ontology/L1/> ;
	skos:definition "The legal entity event activity and processing is in progress." ;
	gleif-base:hasTag "IN_PROGRESS" ;
.

gleif-L1:LegalEntityEventStatusWithdrawnCancelled
	a
		owl:NamedIndividual ,
		gleif-L1:LegalEntityEventStatus ;
	rdfs:label "withdrawn cancelled" ;
	rdfs:isDefinedBy <https://www.gleif.org/ontology/L1/> ;
	skos:definition "The legal entity event as announced will not occur." ;
	gleif-base:hasTag "WITHDRAWN_CANCELLED" ;
.

gleif-L1:LegalEntityEventStatusCompleted
	a
		owl:NamedIndividual ,
		gleif-L1:LegalEntityEventStatus ;
	rdfs:label "completed" ;
	rdfs:isDefinedBy <https://www.gleif.org/ontology/L1/> ;
	skos:definition "The legal entity event activity and processing have been completed as of the LegalEntityEventEffectiveDate." ;
	gleif-base:hasTag "COMPLETED" ;
.

gleif-L1:LegalEntityIdentifier
	a owl:Class ;
	rdfs:subClassOf
		gleif-base:Identifier ,
		[
			a owl:Restriction ;
			owl:onProperty gleif-base:identifies ;
			owl:onClass gleif-L1:RegisteredEntity ;
			owl:qualifiedCardinality "1"^^xsd:nonNegativeInteger ;
		] ,
		[
			a owl:Restriction ;
			owl:onProperty gleif-L1:LEI ;
			owl:onDataRange xsd:string ;
			owl:qualifiedCardinality "1"^^xsd:nonNegativeInteger ;
		]
		;
	rdfs:label "legal entity identifier" ;
	rdfs:isDefinedBy <https://www.gleif.org/ontology/L1/> ;
	skos:definition "The ISO 17442 compatible identifier for the legal entity referenced." ;
	.

gleif-L1:LegalEntityIdentifierRegistryEntry
	a owl:Class ;
	rdfs:subClassOf
		gleif-base:RegistryEntry ,
		[
			a owl:Restriction ;
			owl:onProperty gleif-L1:hasValidationIdentifier ;
			owl:onClass gleif-L1:BusinessRegistryIdentifier ;
			owl:maxQualifiedCardinality "1"^^xsd:nonNegativeInteger ;
		] ,
		[
			a owl:Restriction ;
			owl:onProperty gleif-base:hasNextRenewalDate ;
			owl:maxQualifiedCardinality "1"^^xsd:nonNegativeInteger ;
			owl:onDataRange xsd:dateTime ;
		] ,
		[
			a owl:Restriction ;
			owl:onProperty gleif-L1:hasOtherValidationIdentifier ;
			owl:onClass gleif-L1:BusinessRegistryIdentifier ;
			owl:minQualifiedCardinality "0"^^xsd:nonNegativeInteger ;
		] ,
		[
			a owl:Restriction ;
			owl:onProperty gleif-L1:hasValidationSources ;
			owl:onClass [
				a owl:Class ;
				owl:oneOf (
					gleif-L1:ValidationSourceKindEntitySuppliedOnly
					gleif-L1:ValidationSourceKindFullyCorroborated
					gleif-L1:ValidationSourceKindPartiallyCorroborated
				) ;
			] ;
			owl:minQualifiedCardinality "0"^^xsd:nonNegativeInteger ;
		] ,
		[
			a owl:Restriction ;
			owl:onProperty gleif-L1:hasManagingLOU ;
			owl:onClass gleif-L1:LocalOperatingUnit ;
			owl:qualifiedCardinality "1"^^xsd:nonNegativeInteger ;
		] ,
		[
			a owl:Restriction ;
			owl:onProperty gleif-L1:identifiesAndRecords ;
			owl:onClass gleif-L1:RegisteredEntity ;
			owl:qualifiedCardinality "1"^^xsd:nonNegativeInteger ;
		] ,
		[
			a owl:Restriction ;
			owl:onProperty gleif-base:hasRegistrationStatus ;
			owl:onClass [
				a owl:Class ;
				owl:oneOf (
					gleif-L1:RegistrationStatusAnnulled
					gleif-L1:RegistrationStatusDuplicate
					gleif-L1:RegistrationStatusIssued
					gleif-L1:RegistrationStatusLapsed
					gleif-L1:RegistrationStatusPendingArchival
					gleif-L1:RegistrationStatusPendingTransfer
					gleif-L1:RegistrationStatusRetired
				) ;
			] ;
			owl:qualifiedCardinality "1"^^xsd:nonNegativeInteger ;
		] ,
		[
			a owl:Restriction ;
			owl:onProperty gleif-base:hasInitialRegistrationDate ;
			owl:onDataRange xsd:dateTime ;
			owl:qualifiedCardinality "1"^^xsd:nonNegativeInteger ;
		] ,
		[
			a owl:Restriction ;
			owl:onProperty gleif-base:hasLastUpdateDate ;
			owl:onDataRange xsd:dateTime ;
			owl:qualifiedCardinality "1"^^xsd:nonNegativeInteger ;
		] ,
		[
			a owl:Restriction ;
			owl:onProperty gleif-L1:LEI ;
			owl:onDataRange xsd:string ;
			owl:qualifiedCardinality "1"^^xsd:nonNegativeInteger ;
		]
		;
	rdfs:label "legal entity identifier registry entry" ;
	rdfs:isDefinedBy <https://www.gleif.org/ontology/L1/> ;
	skos:definition "The Registration container element which contains all information on the legal entity's LEI registration with the Managing LOU." ;
	.

gleif-L1:LocalGovernment
	a owl:Class ;
	rdfs:subClassOf gleif-L1:ResidentGovernmentEntity ;
	rdfs:label "local government" ;
	rdfs:isDefinedBy <https://www.gleif.org/ontology/L1/> ;
	skos:altLabel
		"local government entity" 
		;
	skos:definition "The legal entity is a local government subsector which consists of local governments that are separate institutional units." ;
	skos:prefLabel "local government" ;
	.

gleif-L1:LocalOperatingUnit
	a owl:Class ;
	rdfs:subClassOf gleif-L1:LegalEntity ;
	rdfs:label "local operating unit" ;
	rdfs:isDefinedBy <https://www.gleif.org/ontology/L1/> ;
	skos:altLabel
		"LEI issuer" ,
		"LOU"
		;
	skos:definition "An entity that supplies registration, renewal and other services, and acts as the primary interface for legal entities wishing to obtain an LEI. Only organizations duly accredited by the Global Legal Entity Identifier Foundation (GLEIF) are authorized to issue LEIs." ;
	skos:prefLabel "local operating unit" ;
	.

gleif-L1:RegisteredEntity
	a owl:Class ;
	rdfs:subClassOf
		gleif-base:Entity ,
		[
			a owl:Class ;
			owl:complementOf [
				a owl:Class ;
				owl:intersectionOf (
					[
						a owl:Restriction ;
						owl:onProperty gleif-base:hasSuccessor ;
						owl:someValuesFrom gleif-L1:RegisteredEntity ;
					]
					[
						a owl:Restriction ;
						owl:onProperty gleif-base:hasSuccessorName ;
						owl:minCardinality "1"^^xsd:nonNegativeInteger ;
					]
				) ;
			] ;
		] ,
		[
			a owl:Restriction ;
			owl:onProperty gleif-L1:hasLegalName ;
			owl:cardinality "1"^^xsd:nonNegativeInteger ;
		] ,
		[
			a owl:Restriction ;
			owl:onProperty gleif-base:hasSuccessorName ;
			owl:minCardinality "0"^^xsd:nonNegativeInteger ;
		] ,
		[
			a owl:Restriction ;
			owl:onProperty gleif-L1:hasTransliteratedHeadquartersAddress ;
			owl:onClass gleif-base:PhysicalAddressASCII ;
			owl:maxQualifiedCardinality "1"^^xsd:nonNegativeInteger ;
		] ,
		[
			a owl:Restriction ;
			owl:onProperty gleif-L1:hasTransliteratedLegalAddress ;
			owl:onClass gleif-base:PhysicalAddressASCII ;
			owl:maxQualifiedCardinality "1"^^xsd:nonNegativeInteger ;
		] ,
		[
			a owl:Restriction ;
			owl:onProperty gleif-base:hasSuccessor ;
			owl:onClass gleif-L1:LegalEntity ;
			owl:minQualifiedCardinality "0"^^xsd:nonNegativeInteger ;
		] ,
		[
			a owl:Restriction ;
			owl:onProperty gleif-L1:hasOtherEntityNames ;
			owl:minCardinality "0"^^xsd:nonNegativeInteger ;
		] ,
		[
			a owl:Restriction ;
			owl:onProperty gleif-L1:hasOtherAddresses ;
			owl:onClass gleif-base:PhysicalAddress ;
			owl:minQualifiedCardinality "0"^^xsd:nonNegativeInteger ;
		] ,
		[
			a owl:Restriction ;
			owl:onProperty gleif-base:hasEntityStatus ;
			owl:onClass gleif-base:EntityStatus ;
			owl:qualifiedCardinality "1"^^xsd:nonNegativeInteger ;
		] ,
		[
			a owl:Restriction ;
			owl:onProperty gleif-L1:hasHeadquartersAddress ;
			owl:onClass gleif-base:PhysicalAddress ;
			owl:qualifiedCardinality "1"^^xsd:nonNegativeInteger ;
		] ,
		[
			a owl:Restriction ;
			owl:onProperty gleif-L1:hasLegalAddress ;
			owl:onClass gleif-base:PhysicalAddress ;
			owl:qualifiedCardinality "1"^^xsd:nonNegativeInteger ;
		] ,
		[
			a owl:Restriction ;
			owl:onProperty gleif-L1:hasRegistrationIdentifier ;
			owl:onClass gleif-L1:BusinessRegistryIdentifier ;
			owl:qualifiedCardinality "1"^^xsd:nonNegativeInteger ;
		] ,
		[
			a owl:Restriction ;
			owl:onProperty gleif-base:hasLegalJurisdiction ;
			owl:onClass lcc-cr:GeographicRegion ;
			owl:qualifiedCardinality "1"^^xsd:nonNegativeInteger ;
		] ,
		[
			a owl:Restriction ;
			owl:onProperty gleif-base:hasEvent ;
			owl:onClass gleif-base:Event ;
			owl:minQualifiedCardinality "0"^^xsd:nonNegativeInteger ;
		] ,
		[
			owl:intersectionOf (
				[
					a owl:Class ;
					owl:unionOf (
						[
							a owl:Restriction ;
							owl:onProperty gleif-L1:hasLegalForm ;
							owl:onClass gleif-elf:EntityLegalForm ;
							owl:qualifiedCardinality "1"^^xsd:nonNegativeInteger ;
						]
						[
							a owl:Restriction ;
							owl:onProperty gleif-L1:hasLegalFormText ;
							owl:cardinality "1"^^xsd:nonNegativeInteger ;
						]
					) ;
				]
				[
					a owl:Class ;
					owl:complementOf [
						a owl:Class ;
						owl:intersectionOf (
							[
								a owl:Restriction ;
								owl:onProperty gleif-L1:hasLegalForm ;
								owl:someValuesFrom gleif-elf:EntityLegalForm ;
							]
							[
								a owl:Restriction ;
								owl:onProperty gleif-L1:hasLegalFormText ;
								owl:minCardinality "1"^^xsd:nonNegativeInteger ;
							]
						) ;
					] ;
				]
			) ;
		]
		;
	rdfs:label "registered entity" ;
	rdfs:isDefinedBy <https://www.gleif.org/ontology/L1/> ;
	skos:definition "LEI-registered entities including, but not limited to, unique parties that are legally or financially responsible for the performance of financial transactions or have the legal right in their jurisdiction to enter independently into legal contracts, regardless of whether they are incorporated or constituted in some other way (e.g. trust, partnership, contractual). It excludes natural persons, but includes governmental organizations and supranationals." ;
	.

gleif-L1:RegistrationStatus
	a owl:Class ;
	rdfs:subClassOf gleif-base:RegistrationStatus ;
	rdfs:label "legal entity identifier registration status" ;
	rdfs:isDefinedBy <https://www.gleif.org/ontology/L1/> ;
	skos:definition "The status of the legal entity's LEI registration with the Managing LOU." ;
	.

gleif-L1:RegistrationStatusAnnulled
	a
		owl:NamedIndividual ,
		gleif-L1:RegistrationStatus
		;
	rdfs:label "annulled" ;
	rdfs:isDefinedBy <https://www.gleif.org/ontology/L1/> ;
	skos:definition "An LEI registration that was marked as erroneous or invalid after it was issued." ;
	gleif-base:hasTag "ANNULLED" ;
	.

gleif-L1:RegistrationStatusDuplicate
	a
		owl:NamedIndividual ,
		gleif-L1:RegistrationStatus
		;
	rdfs:label "duplicate" ;
	rdfs:isDefinedBy <https://www.gleif.org/ontology/L1/> ;
	skos:definition "An LEI Registration that has been determined to be a duplicate registration of the same legal entity as another LEI Registration; the DUPLICATE status is assigned to the non-surviving registration (i.e. the LEI that should no longer be used)." ;
	gleif-base:hasTag "DUPLICATE" ;
	.

gleif-L1:RegistrationStatusIssued
	a
		owl:NamedIndividual ,
		gleif-L1:RegistrationStatus
		;
	rdfs:label "issued" ;
	rdfs:isDefinedBy <https://www.gleif.org/ontology/L1/> ;
	skos:definition "An LEI Registration that has been validated and issued, and which identifies an entity that was an operating legal entity as of the last update." ;
	gleif-base:hasTag "ISSUED" ;
	.

gleif-L1:RegistrationStatusLapsed
	a
		owl:NamedIndividual ,
		gleif-L1:RegistrationStatus
		;
	rdfs:label "lapsed" ;
	rdfs:isDefinedBy <https://www.gleif.org/ontology/L1/> ;
	skos:definition "An LEI Registration that has not been renewed by the specified next renewal date and is not known by public sources to have ceased operation." ;
	gleif-base:hasTag "LAPSED" ;
	.

gleif-L1:RegistrationStatusMerged
	a
		owl:NamedIndividual ,
		gleif-L1:RegistrationStatus
		;
	rdfs:label "merged" ;
	rdfs:isDefinedBy <https://www.gleif.org/ontology/L1/> ;
	skos:definition "An LEI registration for an entity that has been merged into another legal entity, such that this legal entity no longer exists as an operating entity." ;
	gleif-base:hasTag "MERGED" ;
	owl:deprecated "true"^^xsd:boolean ;
	.

gleif-L1:RegistrationStatusPendingArchival
	a
		owl:NamedIndividual ,
		gleif-L1:RegistrationStatus
		;
	rdfs:label "pending archival" ;
	rdfs:isDefinedBy <https://www.gleif.org/ontology/L1/> ;
	skos:definition "An LEI registration is about to be transferred to a different LOU, after which its registration status will revert to a non-pending status." ;
	gleif-base:hasTag "PENDING_ARCHIVAL" ;
	.

gleif-L1:RegistrationStatusPendingTransfer
	a
		owl:NamedIndividual ,
		gleif-L1:RegistrationStatus
		;
	rdfs:label "pending transfer" ;
	rdfs:isDefinedBy <https://www.gleif.org/ontology/L1/> ;
	skos:definition "An LEI registration that has been requested to be transferred to another LOU. The request is being processed at the sending LOU." ;
	gleif-base:hasTag "PENDING_TRANSFER" ;
	.

gleif-L1:RegistrationStatusRetired
	a
		owl:NamedIndividual ,
		gleif-L1:RegistrationStatus
		;
	rdfs:label "retired" ;
	rdfs:isDefinedBy <https://www.gleif.org/ontology/L1/> ;
	skos:definition "An LEI registration for an entity that has ceased operation, without having been merged into another entity." ;
	gleif-base:hasTag "RETIRED" ;
	.

gleif-L1:ResidentGovernmentEntity
	a owl:Class ;
	rdfs:subClassOf gleif-L1:LegalEntity ;
	rdfs:label "resident government entity" ;
	rdfs:isDefinedBy <https://www.gleif.org/ontology/L1/> ;
	skos:altLabel
		"government entity" 
		;
	skos:definition "The legal entity is a non-market producer, part of a central, state or local government, social security funds or a non-profit institution (NPI) controlled by government units." ;
	skos:prefLabel "resident government entity" ;
	.

gleif-L1:SocialSecurity
	a owl:Class ;
	rdfs:subClassOf gleif-L1:ResidentGovernmentEntity ;
	rdfs:label "social security" ;
	rdfs:isDefinedBy <https://www.gleif.org/ontology/L1/> ;
	skos:altLabel
		"national insurance" 
		;
	skos:definition "The legal entity is a social security scheme which covers a wide variety of programmes, providing benefits in cash or in kind for old age, invalidity or death, survivors, sickness and maternity, work injury, unemployment, family allowance, health care, etc." ;
	skos:prefLabel "social security" ;
	.

gleif-L1:SoleProprietor
	a owl:Class ;
	rdfs:subClassOf gleif-L1:LegalEntity ;
	rdfs:label "sole proprietor" ;
	rdfs:isDefinedBy <https://www.gleif.org/ontology/L1/> ;
	skos:definition "The legal entity represents an individual acting in a business capacity" ;
	.

gleif-L1:StateGovernment
	a owl:Class ;
	rdfs:subClassOf gleif-L1:ResidentGovernmentEntity ;
	rdfs:label "state government" ;
	rdfs:isDefinedBy <https://www.gleif.org/ontology/L1/> ;
	skos:altLabel
		"state government entity" 
		;
	skos:definition "The legal entity is a state government subsector which consists of the institutional units that exercise some government functions at a level below that of the central government and above that of the government institutional units existing at a local level." ;
	skos:prefLabel "state government" ;
	.

gleif-L1:ValidationSourceKind
	a owl:Class ;
	rdfs:label "LEI validation source kind" ;
	rdfs:isDefinedBy <https://www.gleif.org/ontology/L1/> ;
	skos:definition "The level of validation of the reference data provided by the registrant." ;
	.

gleif-L1:ValidationSourceKindEntitySuppliedOnly
	a
		owl:NamedIndividual ,
		gleif-L1:ValidationSourceKind
		;
	rdfs:label "entity supplied only" ;
	rdfs:isDefinedBy <https://www.gleif.org/ontology/L1/> ;
	skos:definition "Based on the validation procedures in use by the LOU responsible for the record, the information associated with this record has significant reliance on the information that a submitter provided due to the unavailability of corroborating information." ;
	gleif-base:hasTag "ENTITY_SUPPLIED_ONLY" ;
	.

gleif-L1:ValidationSourceKindFullyCorroborated
	a
		owl:NamedIndividual ,
		gleif-L1:ValidationSourceKind
		;
	rdfs:label "fully corroborated" ;
	rdfs:isDefinedBy <https://www.gleif.org/ontology/L1/> ;
	skos:definition "Based on the validation procedures in use by the LOU responsible for the record, there is sufficient information contained in authoritative public sources to corroborate the information that the submitter has provided for the record." ;
	gleif-base:hasTag "FULLY_CORROBORATED" ;
	.

gleif-L1:ValidationSourceKindPartiallyCorroborated
	a
		owl:NamedIndividual ,
		gleif-L1:ValidationSourceKind
		;
	rdfs:label "partially corroborated" ;
	rdfs:isDefinedBy <https://www.gleif.org/ontology/L1/> ;
	skos:definition "Based on the validation procedures in use by the LOU responsible for the record, the information supplied by the registrant can be partially corroborated by public authoritative sources, while some of the record is dependent upon the information that the registrant submitted, either due to conflicts with authoritative information, or due to data unavailability." ;
	gleif-base:hasTag "PARTIALLY_CORROBORATED" ;
	.

gleif-L1:hasAlternativeLanguageHeadquartersAddress
	a owl:ObjectProperty ;
	rdfs:subPropertyOf
		gleif-base:hasAddressHeadquarters ,
		gleif-L1:hasOtherAddresses
		;
	rdfs:label "has alternative language headquarters address" ;
	rdfs:isDefinedBy <https://www.gleif.org/ontology/L1/> ;
	skos:definition "Address of the headquarters of the entity, in an alternative language used in the legal jurisdiction." ;
	.

gleif-L1:hasAlternativeLanguageLegalAddress
	a owl:ObjectProperty ;
	rdfs:subPropertyOf
		gleif-base:hasAddressLegal ,
		gleif-L1:hasOtherAddresses
		;
	rdfs:label "has alternative language legal address" ;
	rdfs:isDefinedBy <https://www.gleif.org/ontology/L1/> ;
	skos:definition "Registered address of the entity in the legal jurisdiction, in analternative language used in the legal jurisdiction." ;
	.

gleif-L1:hasAlternativeLanguageLegalName
	a owl:DatatypeProperty ;
	rdfs:subPropertyOf
		gleif-base:hasNameAdditionalLocal ,
		gleif-L1:hasOtherEntityNames
		;
	rdfs:label "has other entity names" ;
	rdfs:isDefinedBy <https://www.gleif.org/ontology/L1/> ;
	skos:definition "Registered name of the entity in an alternative language in the legal jurisdiction in which the entity is registered." ;
	.

gleif-L1:hasAssociatedEntity
	a owl:ObjectProperty ;
	rdfs:label "has associated entity" ;
	rdfs:domain gleif-L1:RegisteredEntity ;
	rdfs:isDefinedBy <https://www.gleif.org/ontology/L1/> ;
	rdfs:range gleif-L1:RegisteredEntity ;
	skos:definition "Another entity associated with this entity if needed to fully identify this entity or to place it in an appropriate context." ;
	owl:deprecated "true"^^xsd:boolean ;
	.

gleif-L1:hasAssociatedEntityName
	a owl:DatatypeProperty ;
	rdfs:label "has associated entity name" ;
	rdfs:domain gleif-L1:RegisteredEntity ;
	rdfs:isDefinedBy <https://www.gleif.org/ontology/L1/> ;
	skos:definition "The name of another entity associated with this entity if needed to fully identify this entity or to place it in an appropriate context." ;
	owl:deprecated "true"^^xsd:boolean ;
	.

gleif-L1:hasAutoASCIITransliteratedHeadquartersAddress
	a owl:ObjectProperty ;
	rdfs:subPropertyOf gleif-L1:hasTransliteratedHeadquartersAddress ;
	rdfs:label "has auto ASCII transliterated headquarters address" ;
	rdfs:isDefinedBy <https://www.gleif.org/ontology/L1/> ;
	skos:definition "Auto transliterated headquarters address for the legal entity." ;
	.

gleif-L1:hasAutoASCIITransliteratedLegalAddress
	a owl:ObjectProperty ;
	rdfs:subPropertyOf gleif-L1:hasTransliteratedLegalAddress ;
	rdfs:label "has auto ASCII transliterated legal address" ;
	rdfs:isDefinedBy <https://www.gleif.org/ontology/L1/> ;
	skos:definition "Auto transliterated legal address for the legal entity." ;
	.

gleif-L1:hasAutoASCIITransliteratedLegalName
	a owl:DatatypeProperty ;
	rdfs:subPropertyOf
		gleif-base:hasNameASCIIAutomatic ,
		gleif-L1:hasTransliteratedOtherEntityNames
		;
	rdfs:label "has auto ASCII transliterated legal name" ;
	rdfs:isDefinedBy <https://www.gleif.org/ontology/L1/> ;
	skos:definition "Legal name of the entity transliterated to ASCII characters, auto-transliterated by the managing LOU." ;
	.

gleif-L1:hasEntityID
	a owl:DatatypeProperty ;
	rdfs:subPropertyOf gleif-base:hasTag ;
	rdfs:label "has entity id" ;
	rdfs:domain gleif-L1:BusinessRegistryIdentifier ;
	rdfs:isDefinedBy <https://www.gleif.org/ontology/L1/> ;
	rdfs:range xsd:string ;
	skos:definition "The identifier of the entity at the indicated registration authority. Typically, the identifier of the legal entity as maintained by a business registry in the jurisdiction of legal registration, or if the entity is one that is not recorded in a business registry (e.g. one of the varieties of funds registered instead with financial regulators), the identifier of the entity in the appropriate registration authority." ;
	.

gleif-L1:hasLegalEntityEventGroupKind
	a owl:ObjectProperty ;
	rdfs:label "has legal entity event group kind" ;
	rdfs:domain gleif-L1:EventGroup ;
	rdfs:isDefinedBy <https://www.gleif.org/ontology/L1/> ;
	rdfs:range gleif-L1:LegalEntityEventGroupKind ;
	skos:definition "The category of the legal entity event group." ;
	.
	
gleif-L1:hasFundFamily
	a owl:ObjectProperty ;
	rdfs:subPropertyOf
		gleif-base:isManagedBy ,
		gleif-L1:hasAssociatedEntity
		;
	rdfs:label "has fund family" ;
	rdfs:domain gleif-L1:Fund ;
	rdfs:isDefinedBy <https://www.gleif.org/ontology/L1/> ;
	rdfs:range gleif-L1:FundFamily ;
	skos:definition "The entity that is the manager of the fund." ;
	owl:deprecated "true"^^xsd:boolean ;
	.

gleif-L1:hasFundFamilyName
	a owl:DatatypeProperty ;
	rdfs:subPropertyOf gleif-L1:hasAssociatedEntityName ;
	rdfs:label "has fund family name" ;
	rdfs:domain gleif-L1:Fund ;
	rdfs:isDefinedBy <https://www.gleif.org/ontology/L1/> ;
	skos:definition "The name of an entity that is the manager of the fund." ;
	owl:deprecated "true"^^xsd:boolean ;
	.

gleif-L1:hasGroupedEvent
	a owl:ObjectProperty ;
	owl:propertyChainAxiom (
		gleif-L1:hasGroupedSequencedEvent
		gleif-L1:hasSequencedEvent
	) ;
	rdfs:label "has grouped event" ;
	rdfs:domain gleif-L1:LegalEntityEventGroup ;
	rdfs:isDefinedBy <https://www.gleif.org/ontology/L1/> ;
	rdfs:range gleif-L1:LegalEntityEvent ;
	skos:definition "The legal entity events that are part of a group of multiple or a complex event." ;
	skos:note "The events may linked direct or via sequenced events." ;
.

gleif-L1:hasGroupedSequencedEvent
	a owl:ObjectProperty ;
	rdfs:label "has grouped sequenced event" ;
	rdfs:domain gleif-L1:LegalEntityEventGroup ;
	rdfs:isDefinedBy <https://www.gleif.org/ontology/L1/> ;
	rdfs:range gleif-L1:LegalEntitySequencedEvent ;
	skos:definition "The legal entity events in sequence that are part of a group of multiple or a complex event."
.

gleif-L1:hasSequencedEvent
	a owl:ObjectProperty ;
	rdfs:label "has sequenced event" ;
	rdfs:domain gleif-L1:LegalEntitySequencedEvent ;
	rdfs:isDefinedBy <https://www.gleif.org/ontology/L1/> ;
	rdfs:range gleif-L1:LegalEntityEvent ;
	skos:definition "The legal entity events in sequence that are part of a group of multiple or a complex event."
.

gleif-L1:hasSequenceNumber
	a owl:DatatypeProperty ;
	rdfs:label "has sequence number" ;
	rdfs:domain gleif-L1:LegalEntitySequencedEvent ;
	rdfs:isDefinedBy <https://www.gleif.org/ontology/L1/> ;
	rdfs:range xsd:positiveInteger ;
	skos:definition "The sequence of one event within a group of multiple or a complex event."
.

gleif-L1:hasHeadquartersAddress
	a owl:ObjectProperty ;
	rdfs:subPropertyOf gleif-base:hasAddressHeadquarters ;
	rdfs:label "has headquarters address" ;
	rdfs:domain gleif-base:Entity ;
	rdfs:isDefinedBy <https://www.gleif.org/ontology/L1/> ;
	rdfs:range gleif-base:PhysicalAddress ;
	skos:definition "The primary address of the headquarters of the Entity." ;
	.

gleif-L1:hasLegalAddress
	a owl:ObjectProperty ;
	rdfs:subPropertyOf gleif-base:hasAddressLegal ;
	rdfs:label "has legal address" ;
	rdfs:domain gleif-base:Entity ;
	rdfs:isDefinedBy <https://www.gleif.org/ontology/L1/> ;
	rdfs:range gleif-base:PhysicalAddress ;
	skos:definition "The primary legal address of the entity as recorded in the registration of the entity in its legal jurisdiction." ;
	.

gleif-L1:hasLegalForm
	a owl:ObjectProperty ;
	rdfs:label "has legal form" ;
	rdfs:domain gleif-base:Entity ;
	rdfs:isDefinedBy <https://www.gleif.org/ontology/L1/> ;
	rdfs:range gleif-elf:EntityLegalForm ;
	skos:definition "The legal form of the entity, taken from the ISO 20275 Entity Legal Form (ELF) data set maintained by GLEIF." ;
	.

gleif-L1:hasLegalFormText
	a owl:DatatypeProperty ;
	rdfs:label "has legal form" ;
	rdfs:domain gleif-base:Entity ;
	rdfs:isDefinedBy <https://www.gleif.org/ontology/L1/> ;
	skos:definition "A legacy code or textual description for the legal entity's legal form, used until a current code from the GLEIF-maintained list can be used." ;
	.

gleif-L1:hasLegalName
	a owl:DatatypeProperty ;
	rdfs:subPropertyOf gleif-base:hasNameLegalLocal ;
	rdfs:label "has legal name" ;
	rdfs:isDefinedBy <https://www.gleif.org/ontology/L1/> ;
	skos:definition "The legal name of the entity." ;
	.

gleif-L1:hasManagingLOU
	a
		owl:ObjectProperty ,
		owl:FunctionalProperty
		;
	rdfs:subPropertyOf gleif-base:isManagedBy ;
	rdfs:label "has managing LOU" ;
	rdfs:domain gleif-base:RegistryEntry ;
	rdfs:isDefinedBy <https://www.gleif.org/ontology/L1/> ;
	rdfs:range gleif-L1:LocalOperatingUnit ;
	skos:definition "The LOU that is responsible for administering this LEI registration." ;
	.

gleif-L1:hasOtherAddresses
	a owl:ObjectProperty ;
	rdfs:subPropertyOf gleif-base:hasAddress ;
	rdfs:label "has other addresses" ;
	rdfs:isDefinedBy <https://www.gleif.org/ontology/L1/> ;
	skos:definition "An optional list of other addresses for the legal entity, excluding transliterations." ;
	.

gleif-L1:hasOtherAuthority
	a owl:DatatypeProperty ;
	rdfs:label "has other authority" ;
	rdfs:domain gleif-L1:BusinessRegistryIdentifier ;
	rdfs:isDefinedBy <https://www.gleif.org/ontology/L1/> ;
	skos:definition "A legacy / historical reference code of a registration authority which is not yet entered in the Registration Authorities List (RAL) maintained by GLEIF, or the designation of an interim register until such time as an entry from RAL can be delivered. " ;
	.

gleif-L1:hasOtherEntityNames
	a owl:DatatypeProperty ;
	rdfs:subPropertyOf gleif-base:hasNameAdditional ;
	rdfs:label "has other entity names" ;
	rdfs:isDefinedBy <https://www.gleif.org/ontology/L1/> ;
	skos:definition "An optional list of other names (excluding transliterations) for the legal entity." ;
	skos:note "Not expected to be used directly: use one of its subProperties." ;
	.

gleif-L1:hasOtherValidationIdentifier
	a owl:ObjectProperty ;
	rdfs:label "has other validation identifier" ;
	rdfs:isDefinedBy <https://www.gleif.org/ontology/L1/> ;
	rdfs:range gleif-base:RegistryIdentifier ;
	skos:altLabel "has additional validation identifier" ;
	skos:definition "An optional list of additional registrations used by the LEI Issuer to validate the entity data." ;
	skos:prefLabel "has other validation identifier" ;
	.

gleif-L1:hasPreferredASCIITransliteratedHeadquartersAddress
	a owl:ObjectProperty ;
	rdfs:subPropertyOf gleif-L1:hasTransliteratedHeadquartersAddress ;
	rdfs:label "has preferred ASCII transliterated headquarters address" ;
	rdfs:isDefinedBy <https://www.gleif.org/ontology/L1/> ;
	skos:definition "Preferred transliterated headquarters address for the legal entity." ;
	.

gleif-L1:hasPreferredASCIITransliteratedLegalAddress
	a owl:ObjectProperty ;
	rdfs:subPropertyOf gleif-L1:hasTransliteratedLegalAddress ;
	rdfs:label "has preferred ASCII transliterated legal address" ;
	rdfs:isDefinedBy <https://www.gleif.org/ontology/L1/> ;
	skos:definition "Preferred transliterated legal address for the legal entity." ;
	.

gleif-L1:hasPreferredASCIITransliteratedLegalName
	a owl:DatatypeProperty ;
	rdfs:subPropertyOf
		gleif-base:hasNameASCIIPreferred ,
		gleif-L1:hasTransliteratedOtherEntityNames
		;
	rdfs:label "has preferred ASCII transliterated legal name" ;
	rdfs:isDefinedBy <https://www.gleif.org/ontology/L1/> ;
	skos:definition "Legal name of the entity transliterated to ASCII characters, provided by the entity for this purpose." ;
	.

gleif-L1:hasPreviousLegalName
	a owl:DatatypeProperty ;
	rdfs:subPropertyOf
		gleif-base:hasNamePreviousLegal ,
		gleif-L1:hasOtherEntityNames
		;
	rdfs:label "has previous legal name" ;
	rdfs:isDefinedBy <https://www.gleif.org/ontology/L1/> ;
	skos:definition "A primary legal name previously used by this entity." ;
	.

gleif-L1:hasRegisteredAuthority
	a owl:ObjectProperty ;
	rdfs:subPropertyOf gleif-base:isRegisteredIn ;
	rdfs:label "has registered authority" ;
	rdfs:domain gleif-L1:BusinessRegistryIdentifier ;
	rdfs:isDefinedBy <https://www.gleif.org/ontology/L1/> ;
	rdfs:range gleif-ra:BusinessRegistry ;
	skos:definition "The reference of the registration authority, taken from the Registration Authorities Code List (RAL) maintained by GLEIF." ;
	.

gleif-L1:hasRegistrationIdentifier
	a owl:ObjectProperty ;
	rdfs:label "has registration identifier" ;
	rdfs:isDefinedBy <https://www.gleif.org/ontology/L1/> ;
	rdfs:range gleif-base:RegistryIdentifier ;
	skos:altLabel
		"has business register entity ID" ,
		"has registration authority"
		;
	skos:definition "An identifier for the legal entity in a business registry in the jurisdiction of legal registration, or in the appropriate registration authority." ;
	skos:prefLabel "has registration identifier" ;
	.

gleif-L1:hasTradingOrOperatingName
	a owl:DatatypeProperty ;
	rdfs:subPropertyOf
		gleif-base:hasNameTradingOrOperating ,
		gleif-L1:hasOtherEntityNames
		;
	rdfs:label "has trading or operating name" ;
	rdfs:isDefinedBy <https://www.gleif.org/ontology/L1/> ;
	skos:altLabel
		"brand name" ,
		"doing business as" ,
		"has trading or operating name" ,
		"operating under" ,
		"trading as"
		;
	skos:definition "A 'trading as', 'brand name' or 'operating under' name currently used by this entity in addition to, but not replacing, the (primary) legal, official registered name" ;
	skos:prefLabel "has trading or operating name" ;
	.

gleif-L1:hasTransliteratedHeadquartersAddress
	a owl:ObjectProperty ;
	rdfs:subPropertyOf
		gleif-base:hasAddressHeadquarters ,
		gleif-L1:hasTransliteratedOtherAddresses
		;
	rdfs:label "has transliterated headquarters address" ;
	rdfs:isDefinedBy <https://www.gleif.org/ontology/L1/> ;
	skos:definition "A transliterated headquarters address for the legal entity." ;
	.

gleif-L1:hasTransliteratedLegalAddress
	a owl:ObjectProperty ;
	rdfs:subPropertyOf
		gleif-base:hasAddressLegal ,
		gleif-L1:hasTransliteratedOtherAddresses
		;
	rdfs:label "has transliterated legal address" ;
	rdfs:isDefinedBy <https://www.gleif.org/ontology/L1/> ;
	skos:definition "A transliterated legal address for the legal entity." ;
	.

gleif-L1:hasTransliteratedOtherAddresses
	a owl:ObjectProperty ;
	rdfs:subPropertyOf gleif-base:hasAddressTransliterated ;
	rdfs:label "has transliterated other addresses" ;
	rdfs:isDefinedBy <https://www.gleif.org/ontology/L1/> ;
	skos:definition "An optional list of transliterated addresses for the legal entity." ;
	.

gleif-L1:hasTransliteratedOtherEntityNames
	a owl:DatatypeProperty ;
	rdfs:subPropertyOf gleif-base:hasNameTransliterated ;
	rdfs:label "has transliterated other entity names" ;
	rdfs:isDefinedBy <https://www.gleif.org/ontology/L1/> ;
	skos:definition "An optional list of ASCII-transliterated (i.e. Latin- or Romanized) representations of names for the legal entity." ;
	skos:note "Not expected to be used directly: use one of its subProperties." ;
	.

gleif-L1:hasValidationIdentifier
	a owl:ObjectProperty ;
	rdfs:label "has validation identifier" ;
	rdfs:isDefinedBy <https://www.gleif.org/ontology/L1/> ;
	rdfs:range gleif-L1:BusinessRegistryIdentifier ;
	skos:altLabel "has validation authority" ;
	skos:definition "The (primary) registration used by the LOU to validate the entity data." ;
	skos:prefLabel "has validation identifier" ;
	.

gleif-L1:hasValidationSources
	a owl:ObjectProperty ;
	rdfs:label "has validation sources" ;
	rdfs:isDefinedBy <https://www.gleif.org/ontology/L1/> ;
	rdfs:range gleif-L1:ValidationSourceKind ;
	skos:definition "The level of validation of the reference data provided by the registrant." ;
	.

gleif-L1:identifiesAndRecords
	a
		owl:ObjectProperty ,
		owl:FunctionalProperty
		;
	rdfs:subPropertyOf
		gleif-base:identifies ,
		gleif-base:records
		;
	rdfs:label "identifies and records" ;
	rdfs:isDefinedBy <https://www.gleif.org/ontology/L1/> ;
	rdfs:range gleif-L1:RegisteredEntity ;
	skos:definition "The legal entity that is recorded by this registry entry and identified by the LEI." ;
	.

[]
	a owl:AllDifferent ;
	owl:members (
		gleif-L1:LegalEntityEventChangeLegalName
		gleif-L1:LegalEntityEventChangeOtherNames
		gleif-L1:LegalEntityEventChangeLegalAddress
		gleif-L1:LegalEntityEventChangeHQAddress
		gleif-L1:LegalEntityEventChangeLegalForm
		gleif-L1:LegalEntityEventDemerger
		gleif-L1:LegalEntityEventSpinoff
		gleif-L1:LegalEntityEventAbsorption
		gleif-L1:LegalEntityEventAcquisitionBranch
		gleif-L1:LegalEntityEventTransformationBranchToSubsidiary
		gleif-L1:LegalEntityEventTransformationSubsidiaryToBranch
		gleif-L1:LegalEntityEventTransformationUmbrellaToStandalone
		gleif-L1:LegalEntityEventBreakup
		gleif-L1:LegalEntityEventMergersAndAcquisitions
		gleif-L1:LegalEntityEventBankruptcy
		gleif-L1:LegalEntityEventLiquidation
		gleif-L1:LegalEntityEventVoluntaryArrangement
		gleif-L1:LegalEntityEventInsolvency
		gleif-L1:LegalEntityEventDissolution
	) ;
	.

[]
	a owl:AllDifferent ;
	owl:members (
		gleif-L1:LegalEntityEventGroupKindReverseTakeover
		gleif-L1:LegalEntityEventGroupKindChangeLegalFormAndName
		gleif-L1:LegalEntityEventGroupKindComplexChangeLegalForm
	) ;
	.

[]
	a owl:AllDifferent ;
	owl:members (
		gleif-L1:LegalEntityEventStatusInProgress
		gleif-L1:LegalEntityEventStatusWithdrawnCancelled
		gleif-L1:LegalEntityEventStatusCompleted
	) ;
	.

[]
	a owl:AllDifferent ;
	owl:members (
		gleif-L1:RegistrationStatusAnnulled
		gleif-L1:RegistrationStatusDuplicate
		gleif-L1:RegistrationStatusIssued
		gleif-L1:RegistrationStatusLapsed
		gleif-L1:RegistrationStatusPendingArchival
		gleif-L1:RegistrationStatusPendingTransfer
		gleif-L1:RegistrationStatusRetired
	) ;
	.

[]
	a owl:AllDifferent ;
	owl:members (
		gleif-L1:ValidationSourceKindEntitySuppliedOnly
		gleif-L1:ValidationSourceKindFullyCorroborated
		gleif-L1:ValidationSourceKindPartiallyCorroborated
	) ;
	.

