# baseURI: https://www.gleif.org/ontology/L1internal/
# imports: https://www.gleif.org/ontology/Base/
# imports: https://www.gleif.org/ontology/L1/

@base <https://www.gleif.org/ontology/L1internal/> .
@prefix dct: <http://purl.org/dc/terms/> .
@prefix gleif-L1: <https://www.gleif.org/ontology/L1/> .
@prefix gleif-L1internal: <https://www.gleif.org/ontology/L1internal/> .
@prefix gleif-base: <https://www.gleif.org/ontology/Base/> .
@prefix owl: <http://www.w3.org/2002/07/owl#> .
@prefix rdf: <http://www.w3.org/1999/02/22-rdf-syntax-ns#> .
@prefix rdfs: <http://www.w3.org/2000/01/rdf-schema#> .
@prefix skos: <http://www.w3.org/2004/02/skos/core#> .
@prefix xml: <http://www.w3.org/XML/1998/namespace> .
@prefix xsd: <http://www.w3.org/2001/XMLSchema#> .

<https://www.gleif.org/ontology/L1internal/>
	a owl:Ontology ;
	rdfs:label "GLEIF L1 Internal Ontology" ;
	dct:abstract "Ontology that builds on GLEIF L1 ontology to add information for LOU internal maintenance purposes." ;
	dct:contributor <https://plus.google.com/+PeteRivett> ;
	dct:creator gleif-base:GLEIF ;
	dct:issued "2019-02-01T00:00:00Z"^^xsd:dateTime ;
	dct:license "https://www.gleif.org/en/meta/lei-data-terms-of-use/"^^xsd:anyURI ;
	dct:rights "Copyright (c) 2019 Global Legal Entity Identifier Foundation (GLEIF)" ;
	dct:rightsHolder gleif-base:GLEIF ;
	dct:title "Global Legal Entity Identifier Foundation Level 1 Ontology - for LOU Internal User"@en ;
	owl:imports
		<https://www.gleif.org/ontology/Base/> ,
		<https://www.gleif.org/ontology/L1/>
		;
	owl:versionIRI <https://www.gleif.org/ontology/L1internal-v1.0/L1internal/> ;
	.

gleif-L1internal:LegalEntityIdentifierRegistryEntry
	a owl:Class ;
	rdfs:subClassOf
		gleif-base:RegistryEntry ,
		[
			a owl:Restriction ;
			owl:onProperty gleif-L1:hasValidationIdentifier ;
			owl:onClass gleif-L1:BusinessRegistryIdentifier ;
			owl:maxQualifiedCardinality "1"^^xsd:nonNegativeInteger ;
		] ,
		[
			a owl:Restriction ;
			owl:onProperty gleif-base:hasNextRenewalDate ;
			owl:maxQualifiedCardinality "1"^^xsd:nonNegativeInteger ;
			owl:onDataRange xsd:dateTime ;
		] ,
		[
			a owl:Restriction ;
			owl:onProperty gleif-L1:hasOtherValidationIdentifier ;
			owl:onClass gleif-L1:BusinessRegistryIdentifier ;
			owl:minQualifiedCardinality "0"^^xsd:nonNegativeInteger ;
		] ,
		[
			a owl:Restriction ;
			owl:onProperty gleif-L1:hasValidationSources ;
			owl:onClass [
				a owl:Class ;
				owl:oneOf (
					gleif-L1:ValidationSourceKindEntitySuppliedOnly
					gleif-L1:ValidationSourceKindFullyCorroborated
					gleif-L1:ValidationSourceKindPartiallyCorroborated
					gleif-L1internal:ValidationSourceKindPending
				) ;
			] ;
			owl:minQualifiedCardinality "1"^^xsd:nonNegativeInteger ;
		] ,
		[
			a owl:Restriction ;
			owl:onProperty gleif-L1:hasManagingLOU ;
			owl:onClass gleif-L1:LocalOperatingUnit ;
			owl:qualifiedCardinality "1"^^xsd:nonNegativeInteger ;
		] ,
		[
			a owl:Restriction ;
			owl:onProperty gleif-L1:identifiesAndRecords ;
			owl:onClass gleif-L1:RegisteredEntity ;
			owl:qualifiedCardinality "1"^^xsd:nonNegativeInteger ;
		] ,
		[
			a owl:Restriction ;
			owl:onProperty gleif-base:hasRegistrationStatus ;
			owl:onClass [
				a owl:Class ;
				owl:oneOf (
					gleif-L1:RegistrationStatusAnnulled
					gleif-L1internal:RegistrationStatusCancelled
					gleif-L1:RegistrationStatusDuplicate
					gleif-L1:RegistrationStatusIssued
					gleif-L1:RegistrationStatusLapsed
					gleif-L1:RegistrationStatusMerged
					gleif-L1:RegistrationStatusPendingArchival
					gleif-L1:RegistrationStatusPendingTransfer
					gleif-L1internal:RegistrationStatusPendingValidation
					gleif-L1:RegistrationStatusRetired
					gleif-L1internal:RegistrationStatusTransferred
				) ;
			] ;
			owl:qualifiedCardinality "1"^^xsd:nonNegativeInteger ;
		] ,
		[
			a owl:Restriction ;
			owl:onProperty gleif-base:hasInitialRegistrationDate ;
			owl:onDataRange xsd:dateTime ;
			owl:qualifiedCardinality "1"^^xsd:nonNegativeInteger ;
		] ,
		[
			a owl:Restriction ;
			owl:onProperty gleif-base:hasLastUpdateDate ;
			owl:onDataRange xsd:dateTime ;
			owl:qualifiedCardinality "1"^^xsd:nonNegativeInteger ;
		]
		;
	rdfs:label "legal entity identifier registry entry" ;
	rdfs:isDefinedBy <https://www.gleif.org/ontology/L1internal/> ;
	skos:definition "The extended Registration container element which contains all information on the legal entity's LEI registration with the Managing LOU." ;
	.

gleif-L1internal:RegistrationStatus
	a owl:Class ;
	rdfs:subClassOf gleif-L1:RegistrationStatus ;
	rdfs:label "registration status" ;
	rdfs:isDefinedBy <https://www.gleif.org/ontology/L1internal/> ;
	owl:oneOf (
		gleif-L1:RegistrationStatusAnnulled
		gleif-L1internal:RegistrationStatusCancelled
		gleif-L1:RegistrationStatusDuplicate
		gleif-L1:RegistrationStatusIssued
		gleif-L1:RegistrationStatusLapsed
		gleif-L1:RegistrationStatusMerged
		gleif-L1:RegistrationStatusPendingArchival
		gleif-L1:RegistrationStatusPendingTransfer
		gleif-L1internal:RegistrationStatusPendingValidation
		gleif-L1:RegistrationStatusRetired
		gleif-L1internal:RegistrationStatusTransferred
	) ;
	skos:definition "The status of the legal entity's LEI registration with the Managing LOU, including internal-only values." ;
	.

gleif-L1internal:RegistrationStatusCancelled
	a
		owl:NamedIndividual ,
		gleif-L1internal:RegistrationStatus
		;
	rdfs:label "cancelled" ;
	rdfs:isDefinedBy <https://www.gleif.org/ontology/L1internal/> ;
	skos:definition "An LEI registration that was abandoned prior to issuance of an LEI." ;
	gleif-base:hasTag "CANCELLED" ;
	.

gleif-L1internal:RegistrationStatusPendingValidation
	a
		owl:NamedIndividual ,
		gleif-L1internal:RegistrationStatus
		;
	rdfs:label "pending validation" ;
	rdfs:isDefinedBy <https://www.gleif.org/ontology/L1internal/> ;
	skos:definition "An application for an LEI that has been submitted and which is being processed and validated." ;
	gleif-base:hasTag "PENDING_VALIDATION" ;
	.

gleif-L1internal:RegistrationStatusTransferred
	a
		owl:NamedIndividual ,
		gleif-L1internal:RegistrationStatus
		;
	rdfs:label "transferred" ;
	rdfs:isDefinedBy <https://www.gleif.org/ontology/L1internal/> ;
	skos:definition "An LEI registration that has been transferred to a different LOU as the managing LOU." ;
	gleif-base:hasTag "TRANSFERRED" ;
	.

gleif-L1internal:ValidationSourceKind
	a owl:Class ;
	rdfs:subClassOf gleif-L1:ValidationSourceKind ;
	rdfs:label "LEI validation source kind" ;
	rdfs:isDefinedBy <https://www.gleif.org/ontology/L1internal/> ;
	owl:oneOf (
		gleif-L1:ValidationSourceKindEntitySuppliedOnly
		gleif-L1:ValidationSourceKindFullyCorroborated
		gleif-L1:ValidationSourceKindPartiallyCorroborated
		gleif-L1internal:ValidationSourceKindPending
	) ;
	skos:definition "The level of validation of the reference data provided by the registrant, including internal-only values." ;
	.

gleif-L1internal:ValidationSourceKindPending
	a
		owl:NamedIndividual ,
		gleif-L1internal:ValidationSourceKind
		;
	rdfs:label "pending" ;
	rdfs:isDefinedBy <https://www.gleif.org/ontology/L1internal/> ;
	skos:definition "The validation of the reference data provided by the registrant has not yet occurred." ;
	gleif-base:hasTag "PENDING" ;
	.

[]
	a owl:AllDifferent ;
	owl:members (
		gleif-L1:RegistrationStatusAnnulled
		gleif-L1internal:RegistrationStatusCancelled
		gleif-L1:RegistrationStatusDuplicate
		gleif-L1:RegistrationStatusIssued
		gleif-L1:RegistrationStatusLapsed
		gleif-L1:RegistrationStatusMerged
		gleif-L1:RegistrationStatusPendingArchival
		gleif-L1:RegistrationStatusPendingTransfer
		gleif-L1internal:RegistrationStatusPendingValidation
		gleif-L1:RegistrationStatusRetired
		gleif-L1internal:RegistrationStatusTransferred
	) ;
	.

[]
	a owl:AllDifferent ;
	owl:members (
		gleif-L1:ValidationSourceKindEntitySuppliedOnly
		gleif-L1:ValidationSourceKindFullyCorroborated
		gleif-L1:ValidationSourceKindPartiallyCorroborated
		gleif-L1internal:ValidationSourceKindPending
	) ;
	.

